More uint63 prim ops + proof of spec

theories/CodegenWasm/LambdaANF_to_Wasm.v
@@ -343,8 +343,7 @@ Definition store_constructor (nenv : name_env) (cenv : ctor_env) (lenv : localva
 (* **** TRANSLATE PRIMITIVE OPERATIONS **** *)
 
 Definition primInt63ModPath : Kernames.modpath :=
-  Kernames.MPfile ["Coq"%bs ; "Numbers"%bs ; "Cyclic"%bs ; "Int63"%bs ; "PrimInt63"%bs ].
-
+  Kernames.MPfile [ "PrimInt63"%bs ; "Int63"%bs ; "Cyclic"%bs ; "Numbers"%bs ; "Coq"%bs ].
 
 Definition primInt63Add  : Kernames.kername := (primInt63ModPath, "add"%bs).
 Definition primInt63Sub  : Kernames.kername := (primInt63ModPath, "sub"%bs).
@@ -356,6 +355,7 @@ Definition primInt63Lor  : Kernames.kername := (primInt63ModPath, "lor"%bs).
 Definition primInt63Lxor : Kernames.kername := (primInt63ModPath, "lxor"%bs).
 Definition primInt63Lsl  : Kernames.kername := (primInt63ModPath, "lsl"%bs).
 Definition primInt63Lsr  : Kernames.kername := (primInt63ModPath, "lsr"%bs).
+Definition primInt63Eqb : Kernames.kername := (primInt63ModPath, "eqb"%bs).
 
 Definition apply_binop_and_store_i64 (op : basic_instruction) y1 y2 :=
   [ BI_global_get global_mem_ptr (* Address to store the result of the operation *)
@@ -380,27 +380,51 @@ Definition translate_primitive_arith_op nenv lenv kname y1 y2 : error (list basi
     y2_var <- translate_var nenv lenv y2 "translate primitive integer arithmetic operation 2nd argument" ;;
     if Kername.eqb kname primInt63Add then
       Ret (apply_binop_and_store_i64 (BI_binop T_i64 (Binop_i BOI_add)) y1_var y2_var)
-          (* else if Kername.eqb kname primInt63Sub then *)
-          (*        Ret (apply_binop_and_store_i64 (BI_binop T_i64 (Binop_i BOI_sub)) y1_var y2_var) *)
-          (* else if Kername.eqb kname primInt63Mul then *)
-          (*        Ret (apply_binop_and_store_i64 (BI_binop T_i64 (Binop_i BOI_mul)) y1_var y2_var) *)
-          (* else if Kername.eqb kname primInt63Div then *)
-          (*        Ret (apply_binop_and_store_i64 (BI_binop T_i64 (Binop_i (BOI_div SX_U))) y1_var y2_var) *)
-          (* else if Kername.eqb kname primInt63Mod then *)
-          (*        Ret (apply_binop_and_store_i64 (BI_binop T_i64 (Binop_i (BOI_rem SX_U))) y1_var y2_var) *)
-          (* else if Kername.eqb kname primInt63Land then *)
-          (*        Ret (apply_binop_and_store_i64 (BI_binop T_i64 (Binop_i BOI_and)) y1_var y2_var) *)
-          (* else if Kername.eqb kname primInt63Lor then *)
-          (*        Ret (apply_binop_and_store_i64 (BI_binop T_i64 (Binop_i BOI_or)) y1_var y2_var) *)
-          (* else if Kername.eqb kname primInt63Lxor then *)
-          (*        Ret (apply_binop_and_store_i64 (BI_binop T_i64 (Binop_i BOI_xor)) y1_var y2_var) *)
-          (* else if Kername.eqb kname primInt63Lsl then *)
-          (*        Ret (apply_binop_and_store_i64 (BI_binop T_i64 (Binop_i BOI_shl)) y1_var y2_var) *)
-          (* else if Kername.eqb kname primInt63Lsr then *)
-          (*        Ret (apply_binop_and_store_i64 (BI_binop T_i64 (Binop_i (BOI_shr SX_U))) y1_var y2_var) *)
+    else if Kername.eqb kname primInt63Sub then
+      Ret (apply_binop_and_store_i64 (BI_binop T_i64 (Binop_i BOI_sub)) y1_var y2_var)
+    else if Kername.eqb kname primInt63Mul then
+      Ret (apply_binop_and_store_i64 (BI_binop T_i64 (Binop_i BOI_mul)) y1_var y2_var)
+    else if Kername.eqb kname primInt63Div then
+      (* Euclidean division *)
+      Ret ([ BI_local_get y2_var
+            ; BI_load T_i64 None 2%N 0%N
+            ; BI_testop T_i64 TO_eqz
+             ; BI_if (BT_valtype None)
+                 [ BI_global_get global_mem_ptr
+                   ; BI_const_num (nat_to_value64 0)
+                   ; BI_store T_i64 None 2%N 0%N ]
+                 [ BI_global_get global_mem_ptr
+                   ; BI_local_get y1_var
+                   ; BI_load T_i64 None 2%N 0%N
+                   ; BI_local_get y2_var
+                   ; BI_load T_i64 None 2%N 0%N
+                   ; BI_binop T_i64 (Binop_i (BOI_div SX_U))
+                   ; BI_store T_i64 None 2%N 0%N ]
+             ; BI_global_get global_mem_ptr
+             ; BI_global_get global_mem_ptr
+             ; BI_const_num (nat_to_value 8)
+             ; BI_binop T_i32 (Binop_i BOI_add)
+             ; BI_global_set global_mem_ptr ])
+    else if Kername.eqb kname primInt63Land then
+      Ret (apply_binop_and_store_i64 (BI_binop T_i64 (Binop_i BOI_and)) y1_var y2_var)
+    else if Kername.eqb kname primInt63Lor then
+      Ret (apply_binop_and_store_i64 (BI_binop T_i64 (Binop_i BOI_or)) y1_var y2_var)
+    else if Kername.eqb kname primInt63Lsl then
+      Ret (apply_binop_and_store_i64 (BI_binop T_i64 (Binop_i BOI_shl)) y1_var y2_var)
+    else if Kername.eqb kname primInt63Lsr then
+      Ret (apply_binop_and_store_i64 (BI_binop T_i64 (Binop_i (BOI_shr SX_U))) y1_var y2_var)
+    else if Kername.eqb kname primInt63Eqb then
+      Ret ([ BI_local_get y1_var
+           ; BI_load T_i64 None 2%N 0%N
+           ; BI_local_get y2_var
+           ; BI_load T_i64 None 2%N 0%N
+           ; BI_relop T_i64 (Relop_i ROI_eq)
+           ; BI_if (BT_valtype (Some (T_num T_i32)))
+               [ BI_const_num (nat_to_value 1) ]
+               [ BI_const_num (nat_to_value 3) ]
+           ])
     else
       Err ("Unknown primitive arithmetic operator: " ++ (Kernames.string_of_kername kname))%bs.
-
 
 Definition translate_primitive_operation (nenv : name_env) (lenv : localvar_env) (x_var : localidx) (p : (kername * string * bool * nat)) (args : list var) : error (list basic_instruction) :=
   let '(kname, _, _, _) := p in
