theories/CodegenWasm/LambdaANF_to_Wasm_correct.v
@@ -36,7 +36,7 @@ From Wasm Require Import datatypes operations host memory_list opsem
                          instantiation_properties properties common numerics.
 
 Require Import Libraries.maps_util.
-From Coq Require Import List Nnat.
+From Coq Require Import List Nnat Uint63.
 
 Import ssreflect eqtype ssrbool eqtype.
 Import LambdaANF.toplevel LambdaANF.cps compM.
@@ -398,7 +398,213 @@ Inductive repr_primitive_operation {lenv} : localidx -> (Kernames.kername * stri
     repr_var (lenv:=lenv) y1 y1' ->
     repr_var (lenv:=lenv) y2 y2' ->
     repr_primitive_operation x (primInt63Add, s, b, n) [y1 ; y2]
-      ((apply_binop_and_store_i64 (BI_binop T_i64 (Binop_i BOI_add)) y1' y2') ++ [:: BI_local_set x])%list.
+      [ BI_global_get global_mem_ptr (* Address to store the result of the operation *)
+                      (* Load the operands onto the stack *)
+        ; BI_local_get y1'
+        ; BI_load T_i64 None 2%N 0%N
+        ; BI_local_get y2'
+        ; BI_load T_i64 None 2%N 0%N
+        ; BI_binop T_i64 (Binop_i BOI_add)
+            (* Bound result of operation to ensure that value fits in 63 bits *)
+        ; BI_const_num (VAL_int64 (Wasm_int.Int64.repr Wasm_int.Int64.half_modulus))
+        ; BI_binop T_i64 (Binop_i (BOI_rem SX_U))
+        ; BI_store T_i64 None 2%N 0%N
+        ; BI_global_get global_mem_ptr (* value to be stored in the let binding ('return value') *)
+                        (* Increment global memory pointer to next free memory segment  *)
+        ; BI_global_get global_mem_ptr
+        ; BI_const_num (nat_to_value 8)
+        ; BI_binop T_i32 (Binop_i BOI_add)
+        ; BI_global_set global_mem_ptr
+        ; BI_local_set x
+      ]
+
+| Rprim_sub :
+  forall x s n y1 y1' y2 y2' b,
+    repr_var (lenv:=lenv) y1 y1' ->
+    repr_var (lenv:=lenv) y2 y2' ->
+    repr_primitive_operation x (primInt63Sub, s, b, n) [y1 ; y2]
+      [ BI_global_get global_mem_ptr (* Address to store the result of the operation *)
+                      (* Load the operands onto the stack *)
+        ; BI_local_get y1'
+        ; BI_load T_i64 None 2%N 0%N
+        ; BI_local_get y2'
+        ; BI_load T_i64 None 2%N 0%N
+        ; BI_binop T_i64 (Binop_i BOI_sub)
+            (* Bound result of operation to ensure that value fits in 63 bits *)
+        ; BI_const_num (VAL_int64 (Wasm_int.Int64.repr Wasm_int.Int64.half_modulus))
+        ; BI_binop T_i64 (Binop_i (BOI_rem SX_U))
+        ; BI_store T_i64 None 2%N 0%N
+        ; BI_global_get global_mem_ptr (* value to be stored in the let binding ('return value') *)
+                        (* Increment global memory pointer to next free memory segment  *)
+        ; BI_global_get global_mem_ptr
+        ; BI_const_num (nat_to_value 8)
+        ; BI_binop T_i32 (Binop_i BOI_add)
+        ; BI_global_set global_mem_ptr
+        ; BI_local_set x
+      ]
+
+| Rprim_mul :
+  forall x s n y1 y1' y2 y2' b,
+    repr_var (lenv:=lenv) y1 y1' ->
+    repr_var (lenv:=lenv) y2 y2' ->
+    repr_primitive_operation x (primInt63Mul, s, b, n) [y1 ; y2]
+      [ BI_global_get global_mem_ptr (* Address to store the result of the operation *)
+                      (* Load the operands onto the stack *)
+        ; BI_local_get y1'
+        ; BI_load T_i64 None 2%N 0%N
+        ; BI_local_get y2'
+        ; BI_load T_i64 None 2%N 0%N
+        ; BI_binop T_i64 (Binop_i BOI_mul)
+            (* Bound result of operation to ensure that value fits in 63 bits *)
+        ; BI_const_num (VAL_int64 (Wasm_int.Int64.repr Wasm_int.Int64.half_modulus))
+        ; BI_binop T_i64 (Binop_i (BOI_rem SX_U))
+        ; BI_store T_i64 None 2%N 0%N
+        ; BI_global_get global_mem_ptr (* value to be stored in the let binding ('return value') *)
+                        (* Increment global memory pointer to next free memory segment  *)
+        ; BI_global_get global_mem_ptr
+        ; BI_const_num (nat_to_value 8)
+        ; BI_binop T_i32 (Binop_i BOI_add)
+        ; BI_global_set global_mem_ptr
+        ; BI_local_set x
+      ]
+| Rprim_div :
+  forall x s n y1 y1' y2 y2' b,
+    repr_var (lenv:=lenv) y1 y1' ->
+    repr_var (lenv:=lenv) y2 y2' ->
+    repr_primitive_operation x (primInt63Div, s, b, n) [y1 ; y2]
+      [ BI_local_get y2'
+        ; BI_load T_i64 None 2%N 0%N
+        ; BI_testop T_i64 TO_eqz
+        ; BI_if (BT_valtype None)
+            [ BI_global_get global_mem_ptr
+              ; BI_const_num (nat_to_value64 0)
+              ; BI_store T_i64 None 2%N 0%N ]
+            [ BI_global_get global_mem_ptr
+              ; BI_local_get y1'
+              ; BI_load T_i64 None 2%N 0%N
+              ; BI_local_get y2'
+              ; BI_load T_i64 None 2%N 0%N
+              ; BI_binop T_i64 (Binop_i (BOI_div SX_U))
+              ; BI_store T_i64 None 2%N 0%N ]
+        ; BI_global_get global_mem_ptr
+        ; BI_global_get global_mem_ptr
+        ; BI_const_num (nat_to_value 8)
+        ; BI_binop T_i32 (Binop_i BOI_add)
+        ; BI_global_set global_mem_ptr
+        ; BI_local_set x
+      ]
+
+| Rprim_land :
+  forall x s n y1 y1' y2 y2' b,
+    repr_var (lenv:=lenv) y1 y1' ->
+    repr_var (lenv:=lenv) y2 y2' ->
+    repr_primitive_operation x (primInt63Land, s, b, n) [y1 ; y2]
+      [ BI_global_get global_mem_ptr (* Address to store the result of the operation *)
+                      (* Load the operands onto the stack *)
+        ; BI_local_get y1'
+        ; BI_load T_i64 None 2%N 0%N
+        ; BI_local_get y2'
+        ; BI_load T_i64 None 2%N 0%N
+        ; BI_binop T_i64 (Binop_i BOI_and)
+            (* Bound result of operation to ensure that value fits in 63 bits *)
+        ; BI_const_num (VAL_int64 (Wasm_int.Int64.repr Wasm_int.Int64.half_modulus))
+        ; BI_binop T_i64 (Binop_i (BOI_rem SX_U))
+        ; BI_store T_i64 None 2%N 0%N
+        ; BI_global_get global_mem_ptr (* value to be stored in the let binding ('return value') *)
+                        (* Increment global memory pointer to next free memory segment  *)
+        ; BI_global_get global_mem_ptr
+        ; BI_const_num (nat_to_value 8)
+        ; BI_binop T_i32 (Binop_i BOI_add)
+        ; BI_global_set global_mem_ptr
+        ; BI_local_set x
+      ]
+| Rprim_lor :
+  forall x s n y1 y1' y2 y2' b,
+    repr_var (lenv:=lenv) y1 y1' ->
+    repr_var (lenv:=lenv) y2 y2' ->
+    repr_primitive_operation x (primInt63Lor, s, b, n) [y1 ; y2]
+      [ BI_global_get global_mem_ptr (* Address to store the result of the operation *)
+                      (* Load the operands onto the stack *)
+        ; BI_local_get y1'
+        ; BI_load T_i64 None 2%N 0%N
+        ; BI_local_get y2'
+        ; BI_load T_i64 None 2%N 0%N
+        ; BI_binop T_i64 (Binop_i BOI_or)
+            (* Bound result of operation to ensure that value fits in 63 bits *)
+        ; BI_const_num (VAL_int64 (Wasm_int.Int64.repr Wasm_int.Int64.half_modulus))
+        ; BI_binop T_i64 (Binop_i (BOI_rem SX_U))
+        ; BI_store T_i64 None 2%N 0%N
+        ; BI_global_get global_mem_ptr (* value to be stored in the let binding ('return value') *)
+                        (* Increment global memory pointer to next free memory segment  *)
+        ; BI_global_get global_mem_ptr
+        ; BI_const_num (nat_to_value 8)
+        ; BI_binop T_i32 (Binop_i BOI_add)
+        ; BI_global_set global_mem_ptr
+        ; BI_local_set x
+      ]
+| Rprim_lsl :
+  forall x s n y1 y1' y2 y2' b,
+    repr_var (lenv:=lenv) y1 y1' ->
+    repr_var (lenv:=lenv) y2 y2' ->
+    repr_primitive_operation x (primInt63Lsl, s, b, n) [y1 ; y2]
+      [ BI_global_get global_mem_ptr (* Address to store the result of the operation *)
+                      (* Load the operands onto the stack *)
+        ; BI_local_get y1'
+        ; BI_load T_i64 None 2%N 0%N
+        ; BI_local_get y2'
+        ; BI_load T_i64 None 2%N 0%N
+        ; BI_binop T_i64 (Binop_i BOI_shl)
+            (* Bound result of operation to ensure that value fits in 63 bits *)
+        ; BI_const_num (VAL_int64 (Wasm_int.Int64.repr Wasm_int.Int64.half_modulus))
+        ; BI_binop T_i64 (Binop_i (BOI_rem SX_U))
+        ; BI_store T_i64 None 2%N 0%N
+        ; BI_global_get global_mem_ptr (* value to be stored in the let binding ('return value') *)
+                        (* Increment global memory pointer to next free memory segment  *)
+        ; BI_global_get global_mem_ptr
+        ; BI_const_num (nat_to_value 8)
+        ; BI_binop T_i32 (Binop_i BOI_add)
+        ; BI_global_set global_mem_ptr
+        ; BI_local_set x
+      ]
+| Rprim_lsr :
+  forall x s n y1 y1' y2 y2' b,
+    repr_var (lenv:=lenv) y1 y1' ->
+    repr_var (lenv:=lenv) y2 y2' ->
+    repr_primitive_operation x (primInt63Lsr, s, b, n) [y1 ; y2]
+      [ BI_global_get global_mem_ptr (* Address to store the result of the operation *)
+                      (* Load the operands onto the stack *)
+        ; BI_local_get y1'
+        ; BI_load T_i64 None 2%N 0%N
+        ; BI_local_get y2'
+        ; BI_load T_i64 None 2%N 0%N
+        ; BI_binop T_i64 (Binop_i (BOI_shr SX_U))
+            (* Bound result of operation to ensure that value fits in 63 bits *)
+        ; BI_const_num (VAL_int64 (Wasm_int.Int64.repr Wasm_int.Int64.half_modulus))
+        ; BI_binop T_i64 (Binop_i (BOI_rem SX_U))
+        ; BI_store T_i64 None 2%N 0%N
+        ; BI_global_get global_mem_ptr (* value to be stored in the let binding ('return value') *)
+                        (* Increment global memory pointer to next free memory segment  *)
+        ; BI_global_get global_mem_ptr
+        ; BI_const_num (nat_to_value 8)
+        ; BI_binop T_i32 (Binop_i BOI_add)
+        ; BI_global_set global_mem_ptr
+        ; BI_local_set x
+      ]
+| Rprim_eqb :
+  forall x s n y1 y1' y2 y2' b,
+    repr_var (lenv:=lenv) y1 y1' ->
+    repr_var (lenv:=lenv) y2 y2' ->
+    repr_primitive_operation x (primInt63Eqb, s, b, n) [y1 ; y2]
+      [ BI_local_get y1'
+        ; BI_load T_i64 None 2%N 0%N
+        ; BI_local_get y2'
+        ; BI_load T_i64 None 2%N 0%N
+        ; BI_relop T_i64 (Relop_i ROI_eq)
+        ; BI_if (BT_valtype (Some (T_num T_i32)))
+            [ BI_const_num (nat_to_value 1) ]
+            [ BI_const_num (nat_to_value 3) ]
+        ; BI_local_set x
+      ].
 
 (* CODEGEN RELATION: relatates LambdaANF expression and result of translate_body *)
 Inductive repr_expr_LambdaANF_Wasm {lenv} : LambdaANF.cps.exp -> list basic_instruction -> Prop :=
@@ -726,7 +932,6 @@ Proof.
     unfold translate_primitive_arith_op in H0.
     destruct (translate_var nenv lenv v0 _) eqn:Hy1. inv H0.
     destruct (translate_var nenv lenv v1 _) eqn:Hy2. inv H0.
-    destruct (Kernames.Kername.eqb k primInt63Add) eqn:Hk. 2: inv H0.
     inv H1.
     eapply R_prim with (p':=(k, t, b, n)) (e':=l0).
     econstructor; eauto.
@@ -736,11 +941,43 @@ Proof.
     }
     now eapply IHe.
     assumption.
+    destruct (Kernames.Kername.eqb k primInt63Add) eqn:HkAdd.
     assert (Hk' : k = primInt63Add) by now apply ReflectEq.eqb_eq.
     inv H0.
-    apply Rprim_add.
-    econstructor; eauto.
-    econstructor; eauto.
+    apply Rprim_add; econstructor; eauto. clear HkAdd.
+    destruct (Kernames.Kername.eqb k primInt63Sub) eqn:HkSub.
+    assert (Hk' : k = primInt63Sub) by now apply ReflectEq.eqb_eq.
+    inv H0.
+    apply Rprim_sub; econstructor; eauto. clear HkSub.
+    destruct (Kernames.Kername.eqb k primInt63Mul) eqn:HkMul.
+    assert (Hk' : k = primInt63Mul) by now apply ReflectEq.eqb_eq.
+    inv H0.
+    apply Rprim_mul; econstructor; eauto.
+    destruct (Kernames.Kername.eqb k primInt63Div) eqn:HkDiv.
+    assert (Hk' : k = primInt63Div) by now apply ReflectEq.eqb_eq.
+    inv H0.
+    apply Rprim_div; econstructor; eauto.
+    destruct (Kernames.Kername.eqb k primInt63Land) eqn:HkLand.
+    assert (Hk' : k = primInt63Land) by now apply ReflectEq.eqb_eq.
+    inv H0.
+    apply Rprim_land; econstructor; eauto.
+    destruct (Kernames.Kername.eqb k primInt63Lor) eqn:HkLor.
+    assert (Hk' : k = primInt63Lor) by now apply ReflectEq.eqb_eq.
+    inv H0.
+    apply Rprim_lor; econstructor; eauto.
+    destruct (Kernames.Kername.eqb k primInt63Lsl) eqn:HkLsl.
+    assert (Hk' : k = primInt63Lsl) by now apply ReflectEq.eqb_eq.
+    inv H0.
+    apply Rprim_lsl; econstructor; eauto.
+    destruct (Kernames.Kername.eqb k primInt63Lsr) eqn:HkLsr.
+    assert (Hk' : k = primInt63Lsr) by now apply ReflectEq.eqb_eq.
+    inv H0.
+    apply Rprim_lsr; econstructor; eauto.
+    destruct (Kernames.Kername.eqb k primInt63Eqb) eqn:HkEqb.
+    assert (Hk' : k = primInt63Eqb) by now apply ReflectEq.eqb_eq.
+    inv H0.
+    apply Rprim_eqb; econstructor; eauto.
+    now inv H0.
   - (* Ehalt *)
     simpl in H. destruct (translate_var nenv lenv v _) eqn:Hvar. inv H.
     injection H => instr'. subst. constructor. now econstructor.
@@ -3273,7 +3510,65 @@ Inductive bs_LambdaANF_prim_fun_extracted_prim_related :
     bs_LambdaANF_prim_fun_extracted_prim_related
       (primInt63Add, s, b, n)
       ( fun vs =>
-          match vs with [ Vprim ( (AstCommon.primInt ; i1) ) ; Vprim ( (AstCommon.primInt ; i2) ) ] => Some ( Vprim (AstCommon.primInt ; (Uint63.add i1 i2) ) ) | _ => None end).
+          match vs with [ Vprim ( (AstCommon.primInt ; i1) ) ; Vprim ( (AstCommon.primInt ; i2) ) ] => Some ( Vprim (AstCommon.primInt ; (Uint63.add i1 i2) ) ) | _ => None end)
+
+| Bstep_primInt_sub : forall s b n (i1 i2 : Uint63.int),
+    bs_LambdaANF_prim_fun_extracted_prim_related
+      (primInt63Sub, s, b, n)
+      ( fun vs =>
+          match vs with [ Vprim ( (AstCommon.primInt ; i1) ) ; Vprim ( (AstCommon.primInt ; i2) ) ] => Some ( Vprim (AstCommon.primInt ; (Uint63.sub i1 i2) ) ) | _ => None end)
+
+| Bstep_primInt_mul : forall s b n (i1 i2 : Uint63.int),
+    bs_LambdaANF_prim_fun_extracted_prim_related
+      (primInt63Mul, s, b, n)
+      ( fun vs =>
+          match vs with [ Vprim ( (AstCommon.primInt ; i1) ) ; Vprim ( (AstCommon.primInt ; i2) ) ] => Some ( Vprim (AstCommon.primInt ; (Uint63.mul i1 i2) ) ) | _ => None end)
+
+| Bstep_primInt_div : forall s b n (i1 i2 : Uint63.int),
+    bs_LambdaANF_prim_fun_extracted_prim_related
+      (primInt63Div, s, b, n)
+      ( fun vs =>
+          match vs with [ Vprim ( (AstCommon.primInt ; i1) ) ; Vprim ( (AstCommon.primInt ; i2) ) ] => Some ( Vprim (AstCommon.primInt ; (Uint63.div i1 i2) ) ) | _ => None end)
+
+| Bstep_primInt_land : forall s b n (i1 i2 : Uint63.int),
+    bs_LambdaANF_prim_fun_extracted_prim_related
+      (primInt63Land, s, b, n)
+      ( fun vs =>
+          match vs with [ Vprim ( (AstCommon.primInt ; i1) ) ; Vprim ( (AstCommon.primInt ; i2) ) ] => Some ( Vprim (AstCommon.primInt ; (Uint63.land i1 i2) ) ) | _ => None end)
+
+| Bstep_primInt_lor : forall s b n (i1 i2 : Uint63.int),
+    bs_LambdaANF_prim_fun_extracted_prim_related
+      (primInt63Lor, s, b, n)
+      ( fun vs =>
+          match vs with [ Vprim ( (AstCommon.primInt ; i1) ) ; Vprim ( (AstCommon.primInt ; i2) ) ] => Some ( Vprim (AstCommon.primInt ; (Uint63.lor i1 i2) ) ) | _ => None end)
+
+| Bstep_primInt_lsl : forall s b n (i1 i2 : Uint63.int),
+    bs_LambdaANF_prim_fun_extracted_prim_related
+      (primInt63Lsl, s, b, n)
+      ( fun vs =>
+          match vs with [ Vprim ( (AstCommon.primInt ; i1) ) ; Vprim ( (AstCommon.primInt ; i2) ) ] => Some ( Vprim (AstCommon.primInt ; (Uint63.lsl i1 i2) ) ) | _ => None end)
+
+| Bstep_primInt_lsr : forall s b n (i1 i2 : Uint63.int),
+    bs_LambdaANF_prim_fun_extracted_prim_related
+      (primInt63Lsr, s, b, n)
+      ( fun vs =>
+          match vs with [ Vprim ( (AstCommon.primInt ; i1) ) ; Vprim ( (AstCommon.primInt ; i2) ) ] => Some ( Vprim (AstCommon.primInt ; (Uint63.lsr i1 i2) ) ) | _ => None end)
+
+| Bstep_primInt_eqb : forall s b n (i1 i2 : Uint63.int) t_true it_true t_false it_false,
+    M.get t_true cenv = Some (Build_ctor_ty_info (Common.BasicAst.nNamed "true") (Common.BasicAst.nNamed "bool") it_true 0%N 0) ->
+    M.get t_false cenv = Some (Build_ctor_ty_info (Common.BasicAst.nNamed "false") (Common.BasicAst.nNamed "bool") it_false 0%N 1) ->
+    bs_LambdaANF_prim_fun_extracted_prim_related
+      (primInt63Eqb, s, b, n)
+      ( fun vs =>
+          match vs with
+          | [ Vprim ( (AstCommon.primInt ; i1) ) ; Vprim ( (AstCommon.primInt ; i2) ) ] =>
+              if Uint63.eqb i1 i2 then
+                Some ( Vconstr t_true [] )
+              else
+                Some ( Vconstr t_false [] )
+          | _ => None
+          end).
+
 
 Definition bs_LambdaANF_prim_fun_env_extracted_prim_env_related (penv : prim_env) (prim_funs : M.t (list val -> option val)) : Prop :=
   forall p p',
@@ -4163,52 +4458,74 @@ Proof.
   now apply Z.eqb_eq.
 Qed.
 
-Lemma wasm_add_prim_add_related :
-  forall w1 w2 w i1 i2,
-    wasm_i64_prim_related w1 (AstCommon.primInt ; i1) ->
-    wasm_i64_prim_related w2 (AstCommon.primInt ; i2) ->
-    Wasm_int.Int64.irem_u (Wasm_int.Int64.iadd w1 w2) (Wasm_int.Int64.repr (Wasm_int.Int64.half_modulus)) = Some w ->
-    wasm_i64_prim_related w (AstCommon.primInt ; (Uint63.add i1 i2)).
+Lemma half_modulus_modulus_range : forall n,
+    (-1 < n < Wasm_int.Int64.half_modulus)%Z ->
+    (-1 < n < Wasm_int.Int64.modulus)%Z.
 Proof.
-  intros ????? Hrel1 Hrel2 Hadd.
-  destruct Hrel1 as [n1 [? [Hn1 [Hw1 [Hi1 Heq1]]]]].
-  destruct Hrel2 as [n2 [? [Hn2 [Hw2 [Hi2 Heq2]]]]].
-  cbn in Hn1, Hn2.
-  assert (i1 = x) by now apply inj_pair2 in Hi1. subst x.
-  assert (i2 = x0) by now apply inj_pair2 in Hi2. subst x0.
-  assert (Hn1Bound : (-1 < n1 < Wasm_int.Int64.modulus)%Z) by now simpl_modulus; simpl.
-  assert (Hn2Bound : (-1 < n2 < Wasm_int.Int64.modulus)%Z) by now simpl_modulus; simpl.
-  assert (Hsum_mod_modulus :
-           (Wasm_int.Int64.Z_mod_modulus ((Wasm_int.Int64.Z_mod_modulus n1) + (Wasm_int.Int64.Z_mod_modulus n2)) = n1 + n2)%Z). {
-    rewrite Wasm_int.Int64.Z_mod_modulus_id. 2: rewrite Wasm_int.Int64.Z_mod_modulus_id; [rewrite Wasm_int.Int64.Z_mod_modulus_id|].
-    rewrite Wasm_int.Int64.Z_mod_modulus_id.
-    rewrite Wasm_int.Int64.Z_mod_modulus_id.
-    all: try lia.
-    simpl_modulus.
-    now simpl.
-  }
-  inversion Hadd as [Hw_eq].
-  have Hw_eq' := Hw_eq.
-  unfold Wasm_int.Int64.modu, Wasm_int.Int64.iadd, Wasm_int.Int64.add in Hw_eq.
-  subst w1 w2.
-  cbn in Hw_eq.
-  rewrite Hsum_mod_modulus in Hw_eq.
-  exists (((n1 + n2) mod 9223372036854775808)%Z), (Uint63.add i1 i2).
-  unfold Wasm_int.Int64.half_modulus, Wasm_int.Int64.modulus, Wasm_int.Int64.wordsize, two_power_nat in *. simpl in *.
-  split. apply Z.mod_pos_bound. cbn. lia.
-  split.
-  unfold Wasm_int.Int64.modu, Wasm_int.Int64.iadd, Wasm_int.Int64.add. simpl. now rewrite Hsum_mod_modulus.
-  split. reflexivity.
-  rewrite Uint63.add_spec.
-  assert (Heq1': (n1 =? Uint63.to_Z i1)%Z = true) by assumption.
-  rewrite Z.eqb_eq in Heq1'.
-  assert (Heq2' :( n2 =? Uint63.to_Z i2)%Z = true) by assumption.
-  rewrite Z.eqb_eq in Heq2'.
-  rewrite Heq1'. rewrite Heq2'.
-  assert (HwB: (9223372036854775808 = Uint63.wB)%Z) by now unfold Uint63.wB.
-  rewrite HwB.
-  now apply Z.eqb_refl.
+  unfold Wasm_int.Int64.half_modulus, Wasm_int.Int64.modulus, two_power_nat in *; cbn in *; lia.
 Qed.
+
+Lemma prim_rel_inv : forall w p p',
+    wasm_i64_prim_related w p ->
+    wasm_i64_prim_related w p' ->
+    p = p'.
+Proof.
+  intros.
+  inv H. destruct H1 as [i [Hx [Hweq [Hpeq Hrel]]]].
+  inv H0. destruct H as [i' [Hx0 [Hweq' [Hpeq' Hrel']]]].
+  assert (x = x0). {
+    apply Wasm_int.Int64.repr_inv.
+    - now apply half_modulus_modulus_range.
+    - now apply half_modulus_modulus_range.
+    - assumption. }
+  subst x0.
+  assert (x =? to_Z i = true)%Z by assumption.
+  assert (x =? to_Z i' = true)%Z by assumption.
+  rewrite Z.eqb_eq in H.  rewrite Z.eqb_eq in H0. rewrite H in H0. apply to_Z_inj in H0. now rewrite -H0 in Hpeq'.
+Qed.
+
+Lemma prim_rel_inv' : forall w w' p,
+    wasm_i64_prim_related w p ->
+    wasm_i64_prim_related w' p ->
+    w = w'.
+Proof.
+  intros.
+  inv H. destruct H1 as [i [Hx [Hweq [Hpeq Hrel]]]].
+  inv H0. destruct H as [i' [Hx0 [Hweq' [Hpeq' Hrel']]]].
+  assert (i = i') by now apply inj_pair2 in Hpeq'. subst i'.
+  assert (x =? to_Z i = true)%Z by assumption.
+  assert (x0 =? to_Z i = true)%Z by assumption.
+  rewrite Z.eqb_eq in H.
+  rewrite Z.eqb_eq in H0.
+  rewrite -H0 in H.
+  now rewrite -H in Hweq'.
+Qed.
+
+
+Lemma repr_var_inv : forall lenv y y' y'',
+    @repr_var nenv lenv y y' ->
+    @repr_var nenv lenv y y'' ->
+    y' = y''.
+Proof.
+  intros. inv H. inv H0. unfold translate_var in H, H1.
+  destruct (lenv ! y) eqn:Hy.
+  - congruence.
+  - discriminate.
+Qed.
+
+Lemma fold_half_modulus :
+  (9223372036854775808 = Wasm_int.Int64.half_modulus)%Z.
+Proof.
+  by now unfold Wasm_int.Int64.half_modulus, Wasm_int.Int64.modulus, two_power_nat.
+Qed.
+
+Ltac simpl_modu H :=
+unfold Wasm_int.Int64.modu in H;
+cbn in H;
+rewrite Wasm_int.Int64.Z_mod_modulus_eq in H;
+rewrite Wasm_int.Int64.modulus_twice_half_modulus in H;
+rewrite fold_half_modulus in H;
+rewrite Zaux.Zmod_mod_mult in H; try lia.
 
 Lemma primitive_operation_reduces : forall lenv pfs state s f m fds f' (x : var) (x' : localidx) (p : prim) p'
  (ys : list var) (e : exp) (vs : list val) (rho : env) (v : val) (gmp_v : u32) instrs,
@@ -4253,398 +4570,993 @@ Proof.
   remember {| f_locs := set_nth (VAL_num (N_to_value gmp_v)) (f_locs f) (N.to_nat x') (VAL_num (N_to_value gmp_v))
            ; f_inst := f_inst f
            |} as fr'.
-
-  inversion HprimRepr. subst.
-  inversion Hys_vs.
-  destruct (rho ! y1) eqn:Hrho_y1. 2: discriminate.
-  destruct (rho ! y2) eqn:Hrho_y2. 2: discriminate.
-  inv H2.
-  have Hpfs' := Hpfs _ _ Hp'.
-  destruct Hpfs' as [f'' [Hf'' Hprimrel]].
-  assert (f' = f'') by congruence.
-  subst f''.
-  inv Hprimrel.
-  destruct v0=>//.
-  destruct p0. destruct x0.
-  destruct v1=>//.
-  destruct p1. destruct x0.
-  inv HprimResSome.
-  clear Hf''.
-  subst.
-  assert (Hin_y1: In y1 [y1 ; y2]) by now constructor.
-  assert (Hin_y2: In y2 [y1 ; y2]) by now right; constructor.
-  assert (HfdsNone_y1: find_def y1 fds = None). {
-    inv H.
-    unfold translate_var in H1.
-    destruct (lenv ! y1) eqn:Hy1. 2: now rewrite Hy1 in H1.
-    unfold domains_disjoint in Hdisjoint.
-    apply Hdisjoint in Hy1.
-    apply HfenvWf_None with (f:=y1) in HfenvWf. now rewrite HfenvWf.
-  }
-  assert (HfdsNone_y2: find_def y2 fds = None). {
-    inv H0.
-    unfold translate_var in H1.
-    destruct (lenv ! y2) eqn:Hy2. 2: now rewrite Hy2 in H1.
-    unfold domains_disjoint in Hdisjoint.
-    apply Hdisjoint in Hy2.
-    apply HfenvWf_None with (f:=y2) in HfenvWf. now rewrite HfenvWf.
-  }
-  have Hy1 := Hlocals _ Hin_y1 HfdsNone_y1. destruct Hy1 as [v1' [w1 [Hrho_y1' [Hloc_y1 Hval_y1]]]].
-  have Hy2 := Hlocals _ Hin_y2 HfdsNone_y2. destruct Hy2 as [v2' [w2 [Hrho_y2' [Hloc_y2 Hval_y2]]]].
-  assert (v1' = Vprim (AstCommon.primInt ; p0)). rewrite Hrho_y1 in Hrho_y1'. now inv Hrho_y1'. subst v1'. clear Hrho_y1'.
-  assert (v2' = Vprim (AstCommon.primInt ; p1)). rewrite Hrho_y2 in Hrho_y2'. now inv Hrho_y2'. subst v2'. clear Hrho_y2'.
-  inversion Hloc_y1 as [? [Htrans Hnth_y1]].
-  assert (x0 = y1'). {
-    inv H.
-    have H' := Htrans err_str.
-    unfold translate_var in H1.
-    unfold translate_var in H'.
-    destruct (lenv ! y1) eqn:Hy1. 2: now rewrite Hy1 in H1.
-    congruence.
-  }
-  subst x0. clear Htrans.
-  inversion Hloc_y2 as [? [Htrans Hnth_y2]].
-  assert (x0 = y2'). {
-    inv H0.
-    have H' := Htrans err_str.
-    unfold translate_var in H1.
-    unfold translate_var in H'.
-    destruct (lenv ! y2) eqn:Hy2. 2: now rewrite Hy2 in H1.
-    congruence.
-  }
-  subst x0. clear Htrans.
-  assert (Hrv1: exists n addr,
-             w1 = Val_ptr addr
-             /\ load_i64 m addr = Some (VAL_int64 n)
-             /\ (wasm_i64_prim_related n (AstCommon.primInt; p0))). {
-    inv Hval_y1.
-    exists w. exists addr. repeat split; auto.
-    replace m with m0 by congruence. auto.
-  }
-  destruct Hrv1 as [n1 [addr1 [Heq1 [Hload1 Hprim_eq1]]]].
-    assert (Hrv2: exists n addr,
-             w2 = Val_ptr addr
-             /\ load_i64 m addr = Some (VAL_int64 n)
-             /\ wasm_i64_prim_related n (AstCommon.primInt ; p1)). {
-    inv Hval_y2.
-    exists w. exists addr. repeat split; auto.
-    replace m with m0 by congruence. auto.
+    have I := Hinv. destruct I as [_ [_ [_ [_ [_ [_ [Hlinmem _]]]]]]].
+    destruct Hlinmem as [Hmem1 [m' [Hmem2 [size [<- [Hmem4 Hmem5]]]]]].
+    assert (m' = m) by congruence. subst m'.
+    assert ((Z.of_N gmp_v < Wasm_int.Int32.modulus)%Z). {
+      apply mem_length_upper_bound in Hmem5. cbn in Hmem5. simpl_modulus. cbn. lia. }
+    assert (exists y1 y2, ys = [ y1 ; y2 ]) by now inv HprimRepr.
+    destruct H0 as [y1 [y2 Hys]].
+    inv Hys_vs.
+    have Hpfs' := Hpfs _ _ Hp'.
+    destruct Hpfs' as [f'' [Hf'' Hprimrel]].
+    assert (f' = f'') by congruence.
+    subst f''.
+    assert (exists v1 v2 p1 i1 p2 i2,
+               rho ! y1 = Some v1 /\ v1 = Vprim p1 /\ p1 = (AstCommon.primInt ; i1)
+               /\ rho ! y2 = Some v2 /\ v2 = Vprim p2 /\ p2 = (AstCommon.primInt ; i2)
+               /\ vs = [ v1 ; v2 ]
+           ). {
+      inv H1.
+      destruct (rho ! y1) eqn:Hrho_y1. 2: discriminate.
+      destruct (rho ! y2) eqn:Hrho_y2. 2: discriminate.
+      rename v0 into v1, v1 into v2.
+      exists v1, v2.
+      inv H2.
+      inv Hprimrel.
+      all: destruct v1=>//.
+      all: destruct p0 eqn:Hp0; destruct x0=>//.
+      all: exists p0, p1.
+      all: destruct v2=>//.
+      all: destruct p2 eqn:Hp2; destruct x0=>//.
+      all: exists p2, p3.
+      all: now split. }
+    destruct H0 as [v1 [v2 [p1 [i1 [p2 [i2 [Hrho_y1 [Heq_v1 [Heq_p1 [Hrho_y2 [Heq_v2 [Heq_p2 Hvs]]]]]]]]]]]].
+    assert (exists y1' y2', repr_var (lenv:=lenv) nenv y1 y1' /\ repr_var (lenv:=lenv) nenv y2 y2'). {
+      inv HprimRepr.
+      all: now exists y1', y2'. }
+    destruct H0 as [y1' [y2' [Hrep_y1 Hrep_y2]]].
+    assert (exists wal1,
+               stored_in_locals (lenv:=lenv) y1 wal1 f /\ repr_val_LambdaANF_Wasm v1 s (f_inst f) wal1). {
+          assert (Hin_y1: In y1 [y1 ; y2]) by now constructor.
+          assert (HfdsNone_y1: find_def y1 fds = None). {
+            inv Hrep_y1.
+            unfold translate_var in H0.
+            destruct (lenv ! y1) eqn:Hy1. 2: now rewrite Hy1 in H0.
+            unfold domains_disjoint in Hdisjoint.
+            apply Hdisjoint in Hy1.
+            apply HfenvWf_None with (f:=y1) in HfenvWf. now rewrite HfenvWf.
+          }
+          have Hy1 := Hlocals _ Hin_y1 HfdsNone_y1. destruct Hy1 as [v1' [w1 [Hrho_y1' [Hloc_y1 Hval_y1]]]].
+          now exists w1.
     }
-    destruct Hrv2 as [n2 [addr2 [Heq2 [Hload2 Hprim_eq2]]]].
-
-  have I := Hinv. destruct I as [_ [_ [_ [_ [_ [_ [Hlinmem _]]]]]]].
-  destruct Hlinmem as [Hmem1 [m' [Hmem2 [size [<- [Hmem4 Hmem5]]]]]].
-  assert (m' = m) by congruence. subst m'.
-  assert ((Z.of_N gmp_v < Wasm_int.Int32.modulus)%Z). {
-    apply mem_length_upper_bound in Hmem5. cbn in Hmem5. simpl_modulus. cbn. lia. }
-  assert (exists n, Wasm_int.Int64.irem_u (Wasm_int.Int64.iadd n1 n2) (Wasm_int.Int64.repr (Wasm_int.Int64.half_modulus)) = Some n ). {
-    destruct Hprim_eq1 as [? [? [? [Hn1 [? He1]]]]]. destruct Hprim_eq2 as [? [? [? [Hn2 [? He2]]]]]. subst.
-    assert (Hn1Bound : (-1 < x0 < Wasm_int.Int64.modulus)%Z). {
-      unfold Wasm_int.Int64.half_modulus, Wasm_int.Int64.modulus, Wasm_int.Int64.wordsize, Wordsize_64.wordsize,  two_power_nat in H2. cbn in H2.
-      unfold Wasm_int.Int64.modulus, Wasm_int.Int64.wordsize, Wordsize_64.wordsize,  two_power_nat. simpl.  now simpl.
+    destruct H0 as [wal1 [Hloc_y1 Hval_y1]].
+    assert (exists wal2,
+               stored_in_locals (lenv:=lenv) y2 wal2 f /\ repr_val_LambdaANF_Wasm v2 s (f_inst f) wal2). {
+      assert (Hin_y2: In y2 [y1 ; y2]) by now right; constructor.
+          assert (HfdsNone_y2: find_def y2 fds = None). {
+            inv Hrep_y2.
+            unfold translate_var in H0.
+            destruct (lenv ! y2) eqn:Hy2. 2: now rewrite Hy2 in H0.
+            unfold domains_disjoint in Hdisjoint.
+            apply Hdisjoint in Hy2.
+            apply HfenvWf_None with (f:=y2) in HfenvWf. now rewrite HfenvWf.
+          }
+          have Hy2 := Hlocals _ Hin_y2 HfdsNone_y2. destruct Hy2 as [v2' [w2 [Hrho_y2' [Hloc_y2 Hval_y2]]]].
+          now exists w2.
     }
-    assert (Hn2Bound : (-1 < x2 < Wasm_int.Int64.modulus)%Z). {
-       unfold Wasm_int.Int64.half_modulus, Wasm_int.Int64.modulus, Wasm_int.Int64.wordsize, Wordsize_64.wordsize,  two_power_nat in H4. cbn in H4.
-      unfold Wasm_int.Int64.modulus, Wasm_int.Int64.wordsize, Wordsize_64.wordsize,  two_power_nat. now simpl.
+    destruct H0 as [wal2 [Hloc_y2 Hval_y2]].
+    destruct Hloc_y1 as [? [Htrans Hy1']].
+    assert (x0 = y1'). {
+      inv Hrep_y1.
+      have H' := Htrans err_str.
+      unfold translate_var in *.
+      destruct (lenv ! y1) eqn:Hy1.
+      congruence.
+      now rewrite Hy1 in H0.
     }
-    assert (Hsum_mod_modulus :
-             (Wasm_int.Int64.Z_mod_modulus ((Wasm_int.Int64.Z_mod_modulus x0) + (Wasm_int.Int64.Z_mod_modulus x2)) = x0 + x2)%Z). {
-      rewrite Wasm_int.Int64.Z_mod_modulus_id. 2: rewrite Wasm_int.Int64.Z_mod_modulus_id; [rewrite Wasm_int.Int64.Z_mod_modulus_id|].
-      rewrite Wasm_int.Int64.Z_mod_modulus_id.
-      rewrite Wasm_int.Int64.Z_mod_modulus_id.
-      all: try lia.
-      unfold Wasm_int.Int64.modulus, Wasm_int.Int64.wordsize, Wordsize_64.wordsize,  two_power_nat. cbn.
-      unfold Wasm_int.Int64.half_modulus, Wasm_int.Int64.modulus, Wasm_int.Int64.wordsize, Wordsize_64.wordsize,  two_power_nat in H2, H4. cbn in H2, H4. lia.
+    subst x0. clear Htrans.
+    destruct Hloc_y2 as [? [Htrans Hy2']].
+    assert (x0 = y2'). {
+      inv Hrep_y2.
+      have H' := Htrans err_str.
+      unfold translate_var in *.
+      destruct (lenv ! y2) eqn:Hy2.
+      congruence.
+      now rewrite Hy2 in H0.
     }
-    exists (Wasm_int.Int64.repr ((x0 + x2) mod Wasm_int.Int64.half_modulus)%Z).
-    cbn.
-    unfold Wasm_int.Int64.modu, Wasm_int.Int64.iadd, Wasm_int.Int64.add.
-    cbn.
-    now rewrite Hsum_mod_modulus.
-  }
-  destruct H2 as [n' Hn'_eq].
-  assert (wasm_i64_prim_related n' (AstCommon.primInt ; (PrimInt63.add p0 p1))) by now apply
-    wasm_add_prim_add_related with (w1:=n1) (w2:=n2).
-  assert (exists mem, store m (Wasm_int.N_of_uint i32m (N_to_i32 gmp_v)) 0%N
-                        (bits (VAL_int64 n'))
-                        8 = Some mem) as Htest.
-  { apply enough_space_to_store. cbn.
-    assert ((Datatypes.length (serialise_i64 n')) = 8) as Hl.
-    { unfold serialise_i64, encode_int, bytes_of_int, rev_if_be.
-      destruct (Archi.big_endian); reflexivity. } rewrite Hl. clear Hl. cbn.
-    rewrite Wasm_int.Int32.Z_mod_modulus_id; try lia.
-    unfold page_size in HenoughM. lia. }
-  destruct Htest as [m' Hm'].
-  remember (upd_s_mem s (set_nth m' s.(s_mems) 0 m')) as s'.
-  assert (Hm'': smem_store s (f_inst f) (Wasm_int.N_of_uint i32m (N_to_i32 gmp_v)) 0%N
-  (VAL_int64 (Wasm_int.Int64.modu (Wasm_int.Int64.iadd n1 n2)
-        (Wasm_int.Int64.repr 9223372036854775808))) T_i64 = Some s'). {
-    unfold smem_store. rewrite Hmem1. cbn. subst s'.
-    unfold smem in Hmem2. rewrite Hmem1 in Hmem2. destruct (s_mems s)=>//.
-    injection Hmem2 as ->. cbn in Hn'_eq. injection Hn'_eq as ->. now rewrite Hm'. }
-
-  assert (Hinv' : INV s' f). {
-    subst.
-    assert (mem_length m = mem_length m'). {
-      apply mem_store_preserves_length in Hm'. congruence. }
-    assert (mem_max_opt m = mem_max_opt m'). {
-      apply mem_store_preserves_max_pages in Hm'. congruence. }
-    eapply update_mem_preserves_INV. apply Hinv. eassumption. erewrite <- H3. lia.
-    congruence. exists (mem_size m); split; auto. unfold mem_size. congruence. reflexivity. }
-  have I := Hinv'. destruct I as [_ [_ [_ [Hgmp_w [_ [_ [Hlinmem' [Hgmp' [_ [_ [_ [_ [_ [Hgmp_mult_two]]]]]]]]]]]]]].
-  destruct (Hgmp_w (Wasm_int.Int32.iadd (N_to_i32 gmp_v) (nat_to_i32 8))) as [s_final Hupd_glob].
-  destruct Hlinmem' as [Hmem1' [m'' [Hmem2' [size' [Hmem3' [Hmem4' Hmem5']]]]]].
-  assert (smem s' (f_inst f) = Some m'). { subst s'. unfold smem, lookup_N. cbn.
-    rewrite Hmem1'. apply set_nth_nth_error_same with (e:=m). unfold smem in Hmem. rewrite Hmem1 in Hmem.
-    destruct (s_mems s)=>//. }
-  assert (m' = m'') by congruence. subst m''.
-  assert (HfsEq: s_funcs s = s_funcs s') by now subst.
-  assert (HfsEq': s_funcs s' = s_funcs s_final) by now apply update_global_preserves_funcs in Hupd_glob.
-  assert (HfsEq'': s_funcs s = s_funcs s_final) by now subst.
-  assert (HgmpBound: (-1 < Z.of_N (gmp_v + 8) < Wasm_int.Int32.modulus)%Z). {
-          apply mem_length_upper_bound in Hmem5. simpl_modulus_in Hmem5. cbn in Hmem5.
-          simpl_modulus. cbn. lia.
-  }
-  remember {| f_locs := set_nth (VAL_num (N_to_value gmp_v)) (f_locs f) (N.to_nat x') (VAL_num (N_to_value gmp_v))
-            ; f_inst := f_inst f
-            |} as f'.
-
-  assert (INV s' f'). {
-    apply update_local_preserves_INV with (f:=f) (x':=N.to_nat x') (v:=N_to_i32 gmp_v).
-    assumption. apply HlocsInBounds with (var:=x). assumption. assumption.
-  }
-
-    assert (HenoughM': (gmp_v + page_size < mem_length m')%N). {
-    assert (mem_length m = mem_length m') by
-      now apply mem_store_preserves_length in Hm'.
-    replace (mem_length m') with (mem_length m). lia. }
-
-  assert (Hinv_final : INV s_final f'). {
-    eapply update_global_preserves_INV with (i:=global_mem_ptr); eauto.
-    { unfold global_mem_ptr, result_out_of_mem. lia. }
-    { subst f'. eassumption. }
-    { move => _.
-      assert ((8 + 8 < Z.of_N page_size)%Z). { unfold page_size. lia. }
-      lia. }
-    { move => _.
-      assert (sglob_val s' (f_inst f) global_mem_ptr =
-                Some (VAL_num (VAL_int32 (N_to_i32 gmp_v)))) by now subst s'.
-      destruct Hgmp_mult_two with (gmp_v:=gmp_v) (m:=m') as [n0 Hn0].
-      assumption. assumption. lia. exists (n0 + 4)%N. lia. }
-    subst f'. cbn.
-    unfold Wasm_int.Int32.iadd, Wasm_int.Int32.add in Hupd_glob.
-    cbn in Hupd_glob.
-    rewrite Wasm_int.Int32.Z_mod_modulus_id in Hupd_glob.
-    assert (Z.of_N gmp_v + 8 = Z.of_N (gmp_v + 8))%Z. lia.
-    unfold N_to_i32. rewrite -H6. assumption.
-    lia.
-  }
-
-  assert (Hrepr_val : repr_val_LambdaANF_Wasm (Vprim (AstCommon.primInt ; (Uint63.add p0 p1))) s_final (f_inst f') (Val_ptr gmp_v)). {
-    apply Rprim_v with (w:=n') (gmp:=(gmp_v+8)%N) (m:=m').
-    { subst f'.
-      cbn.
-      unfold sglob_val, sglob.
-      apply update_global_get_same with (sr:=s') (sr':=s_final).
-      unfold Wasm_int.Int32.iadd, Wasm_int.Int32.add in Hupd_glob. cbn in Hupd_glob.
-      rewrite Wasm_int.Int32.Z_mod_modulus_id in Hupd_glob. unfold N_to_i32.
-      assert (Z.of_N gmp_v + 8 = Z.of_N (gmp_v + 8))%Z. lia. rewrite -H6. assumption. lia. }
-    assumption.
-    lia.
-    assert (sglob_val s' (f_inst f) global_mem_ptr =
-              Some (VAL_num (VAL_int32 (N_to_i32 gmp_v)))) by now subst s'.
-    destruct Hgmp_mult_two with (gmp_v:=gmp_v) (m:=m') as [n0 Hn0].
-    assumption. assumption. lia. exists n0. lia.
-    { unfold supdate_glob, sglob_ind, supdate_glob_s in Hupd_glob.
-      destruct (lookup_N (inst_globals (f_inst f)) global_mem_ptr) eqn:Heq''. 2: discriminate. cbn in Hupd_glob.
-      destruct (lookup_N (s_globals s') g). 2: discriminate.
-      cbn in Hupd_glob. inv Hupd_glob. assumption. }
-    assumption.
-    assert ((wasm_deserialise (bits (VAL_int64 n')) T_i64) = (VAL_int64 n')). {
-      apply deserialise_bits. auto. }
-    rewrite -H6.
-    apply (store_load_i64 m m' gmp_v (bits (VAL_int64 n'))); auto.
-    assert (Wasm_int.N_of_uint i32m (N_to_i32 gmp_v) = gmp_v). {
-      cbn. rewrite Wasm_int.Int32.Z_mod_modulus_id; lia. }
-    rewrite -H7.
-    apply Hm'. }
-
-  assert (HvalsPreserved : forall (wal : wasm_value) (v : val),
-                                      repr_val_LambdaANF_Wasm v s (f_inst f) wal -> repr_val_LambdaANF_Wasm v s_final (f_inst f') wal). {
-    intros.
-    apply val_relation_depends_on_mem_smaller_than_gmp_and_funcs with (sr:=s) (m:=m) (m':=m') (gmp:=gmp_v) (gmp':=(gmp_v + 8)%N); auto.
-    { unfold supdate_glob, sglob_ind, supdate_glob_s in Hupd_glob.
-      destruct (lookup_N (inst_globals (f_inst f)) global_mem_ptr) eqn:Heq''=>//.
-      cbn in Hupd_glob.
-      destruct (lookup_N (s_globals s') g)=>//.
-      cbn in Hupd_glob. injection Hupd_glob as <-. subst. assumption. }
-    { subst s' f'. apply update_global_preserves_memory in Hupd_glob. rewrite -Hupd_glob. assumption. }
-    { subst f'. assumption. }
-    { simpl_modulus. cbn. simpl_modulus_in H1. cbn in H1. simpl_modulus_in HgmpBound.
-      apply mem_length_upper_bound in Hmem5.
-      unfold page_size, max_mem_pages in *. lia. }
-    { subst f'.
-      cbn.
-      unfold sglob_val, sglob.
-      apply update_global_get_same with (sr:=s') (sr':=s_final).
-      unfold Wasm_int.Int32.iadd, Wasm_int.Int32.add in Hupd_glob. cbn in Hupd_glob.
-      rewrite Wasm_int.Int32.Z_mod_modulus_id in Hupd_glob. unfold N_to_i32.
-      assert (Z.of_N gmp_v + 8 = Z.of_N (gmp_v + 8))%Z. lia. rewrite -H7. assumption. lia. }
-    { simpl_modulus. cbn.
-      subst size'.
-      apply mem_length_upper_bound in Hmem5'.
-      unfold page_size, max_mem_pages in *.
-      lia. }
-    lia.
-    { intros.
-      assert (Hv: exists v, load_i32 m a = Some v). { apply enough_space_to_load. subst.
-                                                      simpl_modulus_in HenoughM'. apply mem_store_preserves_length in Hm'. lia. }
-      destruct Hv as [v' Hv'].
-      rewrite Hv'.
-      symmetry.
-      apply (load_store_load_i32' m m' a (Wasm_int.N_of_uint i32m (N_to_i32 gmp_v)) v' (bits (VAL_int64 n'))); auto. cbn. rewrite Wasm_int.Int32.Z_mod_modulus_id; lia. }
-    { intros a Ha.
-      assert (Hex: exists v, load_i64 m a = Some v). {
-        apply enough_space_to_load_i64. lia. }
-      destruct Hex as [v' Hv'].
-      rewrite Hv'. symmetry.
-      apply (load_store_load_i64' m m' a (Wasm_int.N_of_uint i32m (N_to_i32 gmp_v)) v' (bits (VAL_int64 n'))); auto.
-      cbn. rewrite Wasm_int.Int32.Z_mod_modulus_id; lia.
+    subst x0. clear Htrans.
+    assert (Hrv1: exists w1 addr1,
+               wal1 = Val_ptr addr1
+               /\ load_i64 m addr1 = Some (VAL_int64 w1)
+               /\ wasm_i64_prim_related w1 p1). {
+      inv Hval_y1; try discriminate.
+      exists w. exists addr. repeat split; auto.
+      replace m with m0 by congruence. auto.
+      now inv H8.
     }
-    now subst f'.
-  }
-  assert (HrelE' : rel_env_LambdaANF_Wasm (lenv:=lenv) e (M.set x (Vprim (AstCommon.primInt ; (Uint63.add p0 p1))) rho) s_final f' fds). {
-    have Hl := HlocsInBounds _ _ Hrepr_x.
-    apply nth_error_Some in Hl.
-    apply notNone_Some in Hl. destruct Hl as [? Hlx].
-    unfold rel_env_LambdaANF_Wasm.
-    destruct HrelE as [Hfun1 [Hfun2 Hvar]].
-    split.
-    { (* funs1 *)
-      intros ????? Hrho Hv.
-      destruct (var_dec x x1).
-      { (* x = x1 *)
-        subst x1. rewrite M.gss in Hrho. inv Hrho.
-        assert (~ subval_or_eq (Vfun rho' fds' f0) (Vprim (AstCommon.primInt ; (Uint63.add p0 p1)))). { apply subval_or_eq_fun_not_prim. intros. congruence. }
-        contradiction.
+    destruct Hrv1 as [w1 [addr1 [Heq1 [Hload1 Hprim_eq1]]]].
+    assert (Hrv2: exists w2 addr2,
+               wal2 = Val_ptr addr2
+               /\ load_i64 m addr2 = Some (VAL_int64 w2)
+               /\ wasm_i64_prim_related w2 p2). {
+      inv Hval_y2; try discriminate.
+      exists w. exists addr. repeat split; auto.
+      replace m with m0 by congruence. auto.
+      now inv H8.
+    }
+    destruct Hrv2 as [w2 [addr2 [Heq2 [Hload2 Hprim_eq2]]]].
+
+    assert (HloadStep: forall es,
+             reduce_trans
+               (state, s, f, ([:: AI_basic (BI_local_get y1')] ++
+                              [:: AI_basic (BI_load T_i64 None 2%N 0%N)] ++
+                              [:: AI_basic (BI_local_get y2')] ++
+                              [:: AI_basic (BI_load T_i64 None 2%N 0%N)] ++
+                              es))
+               (state, s, f, ([:: $V VAL_num (VAL_int64 w1) ; $V VAL_num (VAL_int64 w2) ] ++ es))). {
+      intros.
+      subst wal1 wal2.
+      unfold load_i64 in Hload1.
+      destruct (load m addr1 0%N 8) eqn:Hload1'. 2: discriminate.
+      assert (addr1 = (Wasm_int.N_of_uint i32m (wasm_value_to_i32 (Val_ptr addr1)))). {
+        cbn. rewrite Wasm_int.Int32.Z_mod_modulus_id. now rewrite N2Z.id.
+        inv Hval_y1; try discriminate. now inv H11. }
+      unfold load_i64 in Hload2.
+      destruct (load m addr2 0%N 8) eqn:Hload2'. 2: discriminate.
+      assert (addr2 = (Wasm_int.N_of_uint i32m (wasm_value_to_i32 (Val_ptr addr2)))). {
+        cbn. rewrite Wasm_int.Int32.Z_mod_modulus_id. now rewrite N2Z.id.
+        inv Hval_y2; try discriminate. now inv H12. }
+      eapply rt_trans with (y := (?[hs], ?[sr], ?[f'], ?[s] ++ ?[t])).
+      apply rt_step.
+      apply r_elimr.
+      apply r_local_get. eassumption.
+      eapply rt_trans with (y := (?[hs], ?[sr], ?[f'], ?[s] ++ ?[t])).
+      apply rt_step.
+      rewrite catA. rewrite cat1s.
+      apply r_elimr. eapply r_load_success; try eassumption. rewrite -H0. apply Hload1'.
+      replace (wasm_deserialise b T_i64) with (VAL_int64 w1) by congruence.
+      eapply rt_trans with (y := (?[hs], ?[sr], ?[f'], ?[s] ++ ?[t])).
+      apply rt_step.
+      apply r_eliml; auto.
+      apply r_elimr.
+      apply r_local_get. eassumption.
+      eapply rt_trans with (y := (?[hs], ?[sr], ?[f'], ?[s] ++ ?[t])).
+      apply rt_step.
+      apply r_eliml; auto.
+      rewrite catA. rewrite cat1s.
+      apply r_elimr. eapply r_load_success; try eassumption. rewrite -H2. apply Hload2'.
+      replace (wasm_deserialise b0 T_i64) with (VAL_int64 w2) by congruence.
+      now apply rt_refl. }
+
+    assert (forall w,
+             exists mem, store m (Wasm_int.N_of_uint i32m (N_to_i32 gmp_v)) 0%N
+                          (bits (VAL_int64 w))
+                          8 = Some mem) as Htest. {
+      intros.
+      apply enough_space_to_store. cbn.
+      assert ((Datatypes.length (serialise_i64 w)) = 8) as Hl.
+      { unfold serialise_i64, encode_int, bytes_of_int, rev_if_be.
+        destruct (Archi.big_endian); reflexivity. } rewrite Hl. clear Hl. cbn.
+      rewrite Wasm_int.Int32.Z_mod_modulus_id; try lia.
+      unfold page_size in HenoughM. lia. }
+
+    assert (forall w pr,   v = Vprim pr ->
+                         wasm_i64_prim_related w pr ->
+                         exists s' s_final fr m' wal,
+              s' = upd_s_mem s (set_nth m' s.(s_mems) 0 m')
+             /\ smem_store s (f_inst f) (Wasm_int.N_of_uint i32m (N_to_i32 gmp_v)) 0%N
+                  (VAL_int64 w) T_i64 = Some s'
+           /\ fr ={| f_locs := set_nth (VAL_num (VAL_int32 (wasm_value_to_i32 wal))) (f_locs f) (N.to_nat x') (VAL_num (VAL_int32 (wasm_value_to_i32 wal)))
+               ; f_inst := f_inst f
+               |}
+           /\ smem s' (f_inst fr) = Some m'
+              /\ reduce_trans (state, s', f, [seq AI_basic i | i <-
+                                                                 [ BI_global_get global_mem_ptr
+                                                                   ; BI_global_get global_mem_ptr
+                                                                   ; BI_const_num (nat_to_value 8)
+                                                                   ; BI_binop T_i32 (Binop_i BOI_add)
+                                                                   ; BI_global_set global_mem_ptr
+                                                                   ; BI_local_set x' ]
+                   ]) (state, s_final, fr, [::])
+
+               /\ INV s' fr
+              /\ supdate_glob s' (f_inst f) global_mem_ptr
+                   (VAL_num (VAL_int32 (Wasm_int.Int32.iadd (N_to_i32 gmp_v) (nat_to_i32 8)))) = Some s_final
+              /\ INV s_final fr
+              /\ f_inst f = f_inst fr
+              /\ s_funcs s = s_funcs s_final
+              /\ rel_env_LambdaANF_Wasm (lenv:=lenv) e (M.set x v rho) s_final fr fds
+              /\ (forall (wal : wasm_value) (v : val),
+                     repr_val_LambdaANF_Wasm v s (f_inst f) wal -> repr_val_LambdaANF_Wasm v s_final (f_inst fr) wal)
+              /\ (exists wal,
+                     fr ={| f_locs := set_nth (VAL_num (VAL_int32 (wasm_value_to_i32 wal))) (f_locs f) (N.to_nat x') (VAL_num (VAL_int32 (wasm_value_to_i32 wal)))
+                            ; f_inst := f_inst f |}
+                     /\ stored_in_locals (lenv:=lenv) x wal fr /\ repr_val_LambdaANF_Wasm v s_final (f_inst fr) wal)
+
+
+
+           ). {
+      intros.
+      destruct (Htest w) as [m' Hm'].
+      remember (upd_s_mem s (set_nth m' s.(s_mems) 0 m')) as s'.
+      exists s'.
+      assert (Hm'': smem_store s (f_inst f) (Wasm_int.N_of_uint i32m (N_to_i32 gmp_v)) 0%N
+                      (VAL_int64 w) T_i64 = Some s'). {
+        unfold smem_store. rewrite Hmem1. cbn. subst s'.
+        unfold smem in Hmem2. rewrite Hmem1 in Hmem2. destruct (s_mems s)=>//.
+        injection Hmem2 as ->. now rewrite Hm'. }
+      assert (Hinv' : INV s' f). {
+        subst.
+        assert (mem_length m = mem_length m'). {
+          apply mem_store_preserves_length in Hm'. congruence. }
+        assert (mem_max_opt m = mem_max_opt m'). {
+          apply mem_store_preserves_max_pages in Hm'. congruence. }
+        eapply update_mem_preserves_INV. apply Hinv. eassumption. erewrite <- H0. lia.
+        congruence. exists (mem_size m); split; auto. unfold mem_size. congruence. reflexivity. }
+      have I := Hinv'. destruct I as [_ [_ [_ [Hgmp_w [_ [_ [Hlinmem' [Hgmp' [_ [_ [_ [_ [_ [Hgmp_mult_two]]]]]]]]]]]]]].
+      destruct (Hgmp_w (Wasm_int.Int32.iadd (N_to_i32 gmp_v) (nat_to_i32 8))) as [s_final Hupd_glob].
+      destruct Hlinmem' as [Hmem1' [m'' [Hmem2' [size' [Hmem3' [Hmem4' Hmem5']]]]]].
+      assert (smem s' (f_inst f) = Some m'). { subst s'. unfold smem, lookup_N. cbn.
+                                               rewrite Hmem1'. apply set_nth_nth_error_same with (e:=m). unfold smem in Hmem. rewrite Hmem1 in Hmem.
+                                               destruct (s_mems s)=>//. }
+      assert (m' = m'') by congruence. subst m''.
+      assert (HfsEq: s_funcs s = s_funcs s') by now subst.
+      assert (HfsEq': s_funcs s' = s_funcs s_final) by now apply update_global_preserves_funcs in Hupd_glob.
+      assert (HfsEq'': s_funcs s = s_funcs s_final) by now subst.
+      assert (HgmpBound: (-1 < Z.of_N (gmp_v + 8) < Wasm_int.Int32.modulus)%Z). {
+        apply mem_length_upper_bound in Hmem5. simpl_modulus_in Hmem5. cbn in Hmem5.
+        simpl_modulus. cbn. lia.
       }
-      { (* x <> x1 *) rewrite M.gso in Hrho; eauto. }
-    } split.
-    { intros ? ? Hnfd. apply Hfun2 with (errMsg:=errMsg) in Hnfd.
-      destruct Hnfd as [i [Htrans Hval]].
-      exists i. split. assumption.
-      apply val_relation_func_depends_on_funcs with (s:=s).
-      assumption.
-      subst f'. assumption.
-    }
-    {
-      intros. destruct (var_dec x x1).
-      { (* x = x1 *)
-        subst x1. exists (Vprim (AstCommon.primInt ; (Uint63.add p0 p1))), (Val_ptr gmp_v).
-        rewrite M.gss. split; auto. (* congruence. split. *)
+      remember {| f_locs := set_nth (VAL_num (N_to_value gmp_v)) (f_locs f) (N.to_nat x') (VAL_num (N_to_value gmp_v))
+               ; f_inst := f_inst f
+               |} as fr.
+
+      assert (INV s' fr). {
+        apply update_local_preserves_INV with (f:=f) (x':=N.to_nat x') (v:=N_to_i32 gmp_v).
+        assumption. apply HlocsInBounds with (var:=x). assumption. assumption.
+      }
+
+      assert (HenoughM': (gmp_v + page_size < mem_length m')%N). {
+        assert (mem_length m = mem_length m') by
+          now apply mem_store_preserves_length in Hm'.
+        replace (mem_length m') with (mem_length m). lia. }
+
+      assert (Hinv_final : INV s_final fr). {
+        eapply update_global_preserves_INV with (i:=global_mem_ptr); eauto.
+        { unfold global_mem_ptr, result_out_of_mem. lia. }
+        { subst fr. eassumption. }
+        { move => _.
+          assert ((8 + 8 < Z.of_N page_size)%Z). { unfold page_size. lia. }
+          lia. }
+        { move => _.
+          assert (sglob_val s' (f_inst f) global_mem_ptr =
+                    Some (VAL_num (VAL_int32 (N_to_i32 gmp_v)))) by now subst s'.
+          destruct Hgmp_mult_two with (gmp_v:=gmp_v) (m:=m') as [n0 Hn0].
+          assumption. assumption. lia. exists (n0 + 4)%N. lia. }
+        subst fr. cbn.
+        unfold Wasm_int.Int32.iadd, Wasm_int.Int32.add in Hupd_glob.
+        cbn in Hupd_glob.
+        rewrite Wasm_int.Int32.Z_mod_modulus_id in Hupd_glob.
+        assert (Z.of_N gmp_v + 8 = Z.of_N (gmp_v + 8))%Z. lia.
+        unfold N_to_i32. rewrite -H6. assumption.
+        lia.
+      }
+
+      assert (Hrepr_val : repr_val_LambdaANF_Wasm v s_final (f_inst fr) (Val_ptr gmp_v)). {
+        subst v.
+        apply Rprim_v with (w:=w) (gmp:=(gmp_v+8)%N) (m:=m').
+        { subst fr.
+          cbn.
+          unfold sglob_val, sglob.
+          apply update_global_get_same with (sr:=s') (sr':=s_final).
+          unfold Wasm_int.Int32.iadd, Wasm_int.Int32.add in Hupd_glob. cbn in Hupd_glob.
+          rewrite Wasm_int.Int32.Z_mod_modulus_id in Hupd_glob. unfold N_to_i32.
+          assert (Z.of_N gmp_v + 8 = Z.of_N (gmp_v + 8))%Z. lia. rewrite -H0. assumption. lia. }
+        assumption.
+        lia.
+        assert (sglob_val s' (f_inst f) global_mem_ptr =
+                  Some (VAL_num (VAL_int32 (N_to_i32 gmp_v)))) by now subst s'.
+        destruct Hgmp_mult_two with (gmp_v:=gmp_v) (m:=m') as [n0 Hn0].
+        assumption. assumption. lia. exists n0. lia.
+        { unfold supdate_glob, sglob_ind, supdate_glob_s in Hupd_glob.
+          destruct (lookup_N (inst_globals (f_inst f)) global_mem_ptr) eqn:Heq''. 2: discriminate. cbn in Hupd_glob.
+          destruct (lookup_N (s_globals s') g). 2: discriminate.
+          cbn in Hupd_glob. inv Hupd_glob. assumption. }
+        assumption.
+        assert ((wasm_deserialise (bits (VAL_int64 w)) T_i64) = (VAL_int64 w)). {
+          apply deserialise_bits. auto. }
+        rewrite -H0.
+        apply (store_load_i64 m m' gmp_v (bits (VAL_int64 w))); auto.
+        assert (Wasm_int.N_of_uint i32m (N_to_i32 gmp_v) = gmp_v). {
+          cbn. rewrite Wasm_int.Int32.Z_mod_modulus_id; lia. }
+        rewrite -H6.
+        apply Hm'. }
+
+
+      assert (HvalsPreserved : forall (wal : wasm_value) (v : val),
+                 repr_val_LambdaANF_Wasm v s (f_inst f) wal -> repr_val_LambdaANF_Wasm v s_final (f_inst fr) wal). {
+        intros.
+        apply val_relation_depends_on_mem_smaller_than_gmp_and_funcs with (sr:=s) (m:=m) (m':=m') (gmp:=gmp_v) (gmp':=(gmp_v + 8)%N); auto.
+        { unfold supdate_glob, sglob_ind, supdate_glob_s in Hupd_glob.
+          destruct (lookup_N (inst_globals (f_inst f)) global_mem_ptr) eqn:Heq''=>//.
+          cbn in Hupd_glob.
+          destruct (lookup_N (s_globals s') g)=>//.
+          cbn in Hupd_glob. injection Hupd_glob as <-. subst. assumption. }
+        { subst s' fr. apply update_global_preserves_memory in Hupd_glob. rewrite -Hupd_glob. assumption. }
+        { subst fr. assumption. }
+        { simpl_modulus. cbn. simpl_modulus_in H1. cbn in H1. simpl_modulus_in HgmpBound.
+          apply mem_length_upper_bound in Hmem5.
+          unfold page_size, max_mem_pages in *. lia. }
+        { subst fr.
+          cbn.
+          unfold sglob_val, sglob.
+          apply update_global_get_same with (sr:=s') (sr':=s_final).
+          unfold Wasm_int.Int32.iadd, Wasm_int.Int32.add in Hupd_glob. cbn in Hupd_glob.
+          rewrite Wasm_int.Int32.Z_mod_modulus_id in Hupd_glob. unfold N_to_i32.
+          assert (Z.of_N gmp_v + 8 = Z.of_N (gmp_v + 8))%Z. lia. rewrite -H7. assumption. lia. }
+        { simpl_modulus. cbn.
+          subst size'.
+          apply mem_length_upper_bound in Hmem5'.
+          unfold page_size, max_mem_pages in *.
+          lia. }
+        lia.
+        { intros.
+          assert (Hex: exists v, load_i32 m a = Some v). {
+            apply enough_space_to_load. subst.
+            simpl_modulus_in HenoughM'.
+            apply mem_store_preserves_length in Hm'. lia. }
+          destruct Hex as [v' Hv'].
+          rewrite Hv'.
+          symmetry.
+          apply (load_store_load_i32' m m' a (Wasm_int.N_of_uint i32m (N_to_i32 gmp_v)) v' (bits (VAL_int64 w))); auto.
+          cbn. rewrite Wasm_int.Int32.Z_mod_modulus_id; lia. }
+        { intros a Ha.
+          assert (Hex: exists v, load_i64 m a = Some v). {
+            apply enough_space_to_load_i64. lia. }
+          destruct Hex as [v' Hv'].
+          rewrite Hv'. symmetry.
+          apply (load_store_load_i64' m m' a (Wasm_int.N_of_uint i32m (N_to_i32 gmp_v)) v' (bits (VAL_int64 w))); auto.
+          cbn. rewrite Wasm_int.Int32.Z_mod_modulus_id; lia.
+        }
+        now subst fr.
+      }
+      assert (HrelE' : rel_env_LambdaANF_Wasm (lenv:=lenv) e (M.set x v rho) s_final fr fds). {
+        have Hl := HlocsInBounds _ _ Hrepr_x.
+        apply nth_error_Some in Hl.
+        apply notNone_Some in Hl. destruct Hl as [? Hlx].
+        unfold rel_env_LambdaANF_Wasm.
+        destruct HrelE as [Hfun1 [Hfun2 Hvar]].
         split.
-        subst f'. exists x'. cbn. split. intros.
-        inv Hrepr_x.  unfold translate_var. unfold translate_var in H8.
-        destruct (lenv ! x) eqn:Hx; rewrite Hx in H8=>//. injection H8 as ->.
-        now rewrite Hx.
-        unfold lookup_N.
-        erewrite set_nth_nth_error_same; eauto.
-        now subst f'.
+        { (* funs1 *)
+          intros ????? Hrho Hv'.
+          destruct (var_dec x x1).
+          { (* x = x1 *)
+            subst x1. rewrite M.gss in Hrho. inv Hrho.
+            assert (~ subval_or_eq (Vfun rho' fds' f0) (Vprim pr)). { apply subval_or_eq_fun_not_prim. intros. congruence. }
+            contradiction.
+          }
+          { (* x <> x1 *) rewrite M.gso in Hrho; eauto. }
+        } split.
+        { intros ? ? Hnfd. apply Hfun2 with (errMsg:=errMsg) in Hnfd.
+          destruct Hnfd as [i' [Htrans Hval]].
+          exists i'. split. assumption.
+          apply val_relation_func_depends_on_funcs with (s:=s).
+          assumption.
+          subst fr. assumption.
+        }
+        {
+          intros. destruct (var_dec x x1).
+          { (* x = x1 *)
+            subst x1. exists v, (Val_ptr gmp_v).
+            rewrite M.gss. split; auto. (* congruence. split. *)
+            split.
+            subst fr. exists x'. cbn. split. intros.
+            inv Hrepr_x.  unfold translate_var. unfold translate_var in H8.
+            destruct (lenv ! x) eqn:Hx; rewrite Hx in H8=>//. injection H8 as ->.
+            now rewrite Hx.
+            unfold lookup_N.
+            erewrite set_nth_nth_error_same; eauto.
+            now subst fr.
+          }
+          { (* x <> x1 *)
+            assert (Hocc : occurs_free (Eprim x p [ y1 ; y2 ] e) x1) by now apply Free_Eprim2.
+            have H' := Hvar _ Hocc H7.
+            destruct H' as [val' [wal' [Hrho [Hloc Hval]]]].
+            exists val', wal'. split.
+            rewrite M.gso; auto. split.
+            destruct Hloc as [i' [Hl1 Hl2]].
+            unfold stored_in_locals. exists i'. split; auto.
+            subst fr. unfold lookup_N.
+            rewrite set_nth_nth_error_other; auto.
+            inv Hrepr_x.
+            specialize Hl1 with err_str.
+            intro. assert (x' = i') by lia. subst x'.
+            unfold translate_var in Hl1, H8.
+            destruct (lenv ! x1) eqn:Hlx1; rewrite Hlx1 in Hl1=>//.
+            destruct (lenv ! x) eqn:Hlx2; rewrite Hlx2 in H8=>//.
+            have H'' := HlenvInjective _ _ _ _ n Hlx2 Hlx1. congruence.
+            apply nth_error_Some. congruence.
+            now apply HvalsPreserved.
+          }
+        }
       }
-      { (* x <> x1 *)
-        assert (Hocc : occurs_free (Eprim x p [ y1 ; y2 ] e) x1) by now apply Free_Eprim2.
-        have H' := Hvar _ Hocc H7.
-        destruct H' as [val' [wal' [Hrho [Hloc Hval]]]].
-        exists val', wal'. split.
-        rewrite M.gso; auto. split.
-        destruct Hloc as [i [Hl1 Hl2]].
-        unfold stored_in_locals. exists i. split; auto.
-        subst f'. unfold lookup_N.
-        rewrite set_nth_nth_error_other; auto.
-        inv Hrepr_x.
-        specialize Hl1 with err_str.
-        intro. assert (x' = i) by lia. subst x'.
-        unfold translate_var in Hl1, H8.
-        destruct (lenv ! x1) eqn:Hlx1; rewrite Hlx1 in Hl1=>//.
-        destruct (lenv ! x) eqn:Hlx2; rewrite Hlx2 in H8=>//.
-        have H'' := HlenvInjective _ _ _ _ n0 Hlx2 Hlx1. congruence.
-        apply nth_error_Some. congruence.
-        now apply HvalsPreserved.
+      exists s_final, fr, m', (Val_ptr gmp_v).
+      split. assumption. (* assert (pr = pi) by congruence.  *) (* now rewrite H4 in Hrel. *)
+      split. assumption.
+      split. now subst fr.
+      split. now subst fr.
+      split. {
+        assert (sglob_val s' (f_inst f) global_mem_ptr =
+                  Some (VAL_num (VAL_int32 (N_to_i32 gmp_v)))) by now subst s'.
+        separate_instr.
+        dostep_nary 0. eapply r_global_get.
+        eassumption.
+        dostep. apply r_eliml. auto.
+        elimr_nary_instr 0. apply r_global_get. eassumption.
+        dostep. apply r_eliml. auto.
+        elimr_nary_instr 2. constructor. apply rs_binop_success. reflexivity.
+        dostep. apply r_eliml. auto.
+        elimr_nary_instr 1. apply r_global_set with (v:=VAL_num (VAL_int32 (Wasm_int.Int32.iadd (N_to_i32 gmp_v) (nat_to_i32 8)))). eassumption.
+        apply rt_step. cbn.
+        assert ($VN VAL_int32 (N_to_i32 gmp_v) = $V (VAL_num (N_to_value gmp_v))). auto.
+        rewrite H7.
+        eapply r_local_set. now subst fr.
+        apply /ssrnat.leP.
+        apply HlocsInBounds in Hrepr_x. lia.
+        now subst fr. }
+      split. assumption.
+      split. assumption.
+      split. assumption.
+      split. now subst fr.
+      split. assumption.
+      split. assumption.
+      split.
+      assumption.
+      exists (Val_ptr gmp_v).
+      split. assumption.
+      split. {
+        unfold stored_in_locals. exists x'. split. intros. inv Hrepr_x. unfold translate_var. unfold translate_var in H6. destruct (lenv ! x) eqn:Hx. rewrite Hx in H6. rewrite Hx. congruence. now rewrite Hx in H6.
+        subst fr. cbn. unfold lookup_N.
+        apply nth_error_set_eq. }
+      assumption. }
+
+    assert (forall t ord, v = Vconstr t [] ->
+                          get_ctor_arity cenv t = Ret 0 ->
+                      get_ctor_ord cenv t = Ret ord ->
+                         exists fr wal,
+                           INV s fr
+                           /\ fr = {| f_locs := set_nth (VAL_num (VAL_int32 (wasm_value_to_i32 wal))) (f_locs f) (N.to_nat x') (VAL_num (VAL_int32 (wasm_value_to_i32 wal)))
+               ; f_inst := f_inst f
+               |}
+                           /\ repr_val_LambdaANF_Wasm v s (f_inst fr) wal
+                           /\ rel_env_LambdaANF_Wasm (lenv:=lenv) e (M.set x v rho) s fr fds
+                           /\ (forall (wal0 : wasm_value) (v : val),
+                                  repr_val_LambdaANF_Wasm v s (f_inst f) wal0 -> repr_val_LambdaANF_Wasm v s (f_inst fr) wal0)
+                           /\ reduce_trans (state, s, f, [ (v_to_e (VAL_num (VAL_int32 (wasm_value_to_i32 wal))))
+                                                                       ; AI_basic (BI_local_set x') ]
+                                ) (state, s, fr, [::])). {
+      intros.
+      remember {| f_locs := set_nth (VAL_num (N_to_value (2 * ord + 1))) (f_locs f) (N.to_nat x') (VAL_num (N_to_value (2 * ord + 1)))
+               ; f_inst := f_inst f
+               |} as fr.
+      assert (Hinv' : INV s fr). {
+        apply update_local_preserves_INV with (f:=f) (x':=N.to_nat x') (v:=(N_to_i32 (2 * ord + 1))).
+        assumption.
+        apply HlocsInBounds with (var:=x). assumption.
+        now subst fr. }
+
+      assert (HvalsPreserved:
+               (forall (wal0 : wasm_value) (v0 : val),
+                   repr_val_LambdaANF_Wasm v0 s (f_inst f) wal0 -> repr_val_LambdaANF_Wasm v0 s (f_inst fr) wal0)) by now subst fr.
+
+      assert (HreprVal: repr_val_LambdaANF_Wasm v s (f_inst fr) (Val_unboxed (2 * ord + 1)%N)). {
+        rewrite H2.
+        have H' := Uint63.eq_dec i1 i2.
+        inv Hprimrel; try inv HprimResSome.
+        destruct H' as [H'|H'].
+        apply Uint63.eqb_complete in H'. rewrite H' in H7.
+        assert (t = t_true) by congruence.
+        apply Rconstr_unboxed_v with (ord:=ord).
+        assumption.
+        now rewrite N.mul_comm.
+        assert (ord = 0%N). inv H7. unfold get_ctor_ord in H4. rewrite H5 in H4. now inv H4.
+        simpl_modulus. subst ord. cbn. lia. assumption.
+        apply Uint63.eqb_false_complete in H'. rewrite H' in H7.
+        assert (t = t_false) by congruence. subst t.
+        apply Rconstr_unboxed_v with (ord:=ord).
+        assumption.
+        now rewrite N.mul_comm.
+        assert (ord = 1%N). inv H7. unfold get_ctor_ord in H4. rewrite H6 in H4. now inv H4.
+        simpl_modulus. subst ord. cbn. lia. assumption.
       }
-    }
-  }
 
-  exists s_final. exists f'.
-  split.
-  separate_instr.
-  dostep_nary 0. apply r_global_get. eassumption.
-  dostep. apply r_eliml. auto.
-  elimr_nary_instr 0. apply r_local_get. eassumption.
-  unfold load_i64 in Hload1.
-  destruct (load m addr1 0%N 8) eqn:Hload. 2: discriminate.
-  assert (addr1 = (Wasm_int.N_of_uint i32m (wasm_value_to_i32 w1))). {
-    cbn. rewrite Wasm_int.Int32.Z_mod_modulus_id.
-    subst w1. cbn. lia. cbn.
-    inv Hval_y1; try discriminate.
-    cbn. inv H16. lia.
-  }
-  dostep. apply r_eliml. auto.
-  elimr_nary_instr 1. eapply r_load_success; try eassumption.
-  rewrite <- H6. cbn. apply Hload.
-  replace (wasm_deserialise b0 T_i64) with (VAL_int64 n1) by congruence.
-  dostep. apply r_eliml. auto. apply r_eliml. auto.
-  elimr_nary_instr 0. apply r_local_get. eassumption.
-  unfold load_i64 in Hload2.
-  destruct (load m addr2 0%N 8) eqn:Hload'. 2: discriminate.
-  assert (addr2 = (Wasm_int.N_of_uint i32m (wasm_value_to_i32 w2))). {
-    cbn. rewrite Wasm_int.Int32.Z_mod_modulus_id.
-    subst w2. cbn. lia. cbn.
-    inv Hval_y2; try discriminate.
-    cbn. inv H17. lia.
-  }
-  dostep. apply r_eliml. auto. apply r_eliml. auto.
-  elimr_nary_instr 1. eapply r_load_success; try eassumption.
-  rewrite <- H7. apply Hload'.
-  replace (wasm_deserialise b1 T_i64) with (VAL_int64 n2) by congruence.
-  dostep. apply r_eliml. auto.
-  elimr_nary_instr 2. constructor. apply rs_binop_success. reflexivity.
-  dostep. apply r_eliml. auto.
-  elimr_nary_instr 2. constructor. apply rs_binop_success. cbn. cbn in Hn'_eq. inv Hn'_eq. reflexivity.
-  dostep.
-  elimr_nary_instr 2. eapply r_store_success.
-  inv Hn'_eq. eapply Hm''.
-  dostep_nary 0. apply r_global_get. eassumption.
-  dostep. apply r_eliml. auto.
-  elimr_nary_instr 0. apply r_global_get. eassumption.
-  dostep. apply r_eliml. auto.
-  elimr_nary_instr 2. constructor. apply rs_binop_success. reflexivity.
-  dostep. apply r_eliml. auto.
-  elimr_nary_instr 1. apply r_global_set with (v:=VAL_num (VAL_int32 (Wasm_int.Int32.iadd (N_to_i32 gmp_v) (nat_to_i32 8)))). subst s'. eassumption.
-  rewrite cat0s.
-  constructor. eapply r_local_set with (v:=VAL_num (VAL_int32 (N_to_i32 gmp_v))). subst. reflexivity.
-  apply /ssrnat.leP.
-  apply HlocsInBounds in Hrepr_x. lia.
-  subst f'. cbn. reflexivity.
-  split. assumption.
-  split. now subst f'.
-  split. assumption.
-  split. assumption.
-  split. assumption.
-  exists (Val_ptr gmp_v). split. now subst f'.
-  split.
-  exists x'. split. intros. inv Hrepr_x.
-  unfold translate_var in H6. unfold translate_var.
-  destruct (lenv ! x) eqn:Hx;rewrite Hx in H6=>//. now rewrite Hx.
-  subst f'. cbn. unfold nat_to_value, nat_to_i32, wasm_value_to_i32, wasm_value_to_u32.
+      assert (HrelE' : @rel_env_LambdaANF_Wasm lenv e (map_util.M.set x v rho) s fr fds). {
+        have Hl := HlocsInBounds _ _ Hrepr_x.
+        apply nth_error_Some in Hl.
+        apply notNone_Some in Hl. destruct Hl as [? Hlx].
 
-  have Hl := HlocsInBounds _ _ Hrepr_x.
-  apply nth_error_Some in Hl.
-  apply notNone_Some in Hl. destruct Hl as [? Hlx].
-  unfold lookup_N.
-  erewrite set_nth_nth_error_same; try eassumption.
-  reflexivity. assumption.
-  discriminate.
-  discriminate.
+        destruct HrelE as [Hfun1 [Hfun2 Hvar]]. unfold rel_env_LambdaANF_Wasm. split.
+        { intros. destruct (var_dec x x1).
+          { subst x1. rewrite M.gss in H5. inv H5.
+            apply subval_or_eq_fun in H6.
+            destruct H6 as [v1 [Hr1 Hr2]]. inv Hr2.
+          }
+          { by rewrite M.gso in H5; eauto. }
+        } split.
+        { intros ? ? Hnfd. apply Hfun2 with (errMsg:=errMsg) in Hnfd.
+          destruct Hnfd as [i [Htrans Hval]].
+          exists i. split. assumption. now subst fr.
+        }
+        { intros. destruct (var_dec x x1).
+          { subst x1.
+
+            assert ( (Wasm_int.Int32.half_modulus < Wasm_int.Int32.modulus)%Z ) by now rewrite Wasm_int.Int32.half_modulus_modulus.
+            exists (Vconstr t []), (Val_unboxed (2 * ord + 1)%N).
+            rewrite M.gss. split. congruence.
+            split.
+            {
+              unfold stored_in_locals. exists x'. split.
+              - unfold translate_var. inv Hrepr_x. unfold translate_var in H8.
+                destruct (lenv ! x) eqn:Hx; rewrite Hx in H8=>//. injection H8 as ->. now rewrite Hx.
+              - subst fr. unfold lookup_N, nat_to_value, nat_to_i32, wasm_value_to_i32. simpl.
+                erewrite set_nth_nth_error_same; eauto.
+            }
+            {
+              econstructor ; eauto.
+              now rewrite N.mul_comm.
+              {
+                now inv HreprVal. }
+              }
+            }
+          {
+            assert (Hocc: occurs_free (Eprim x p [:: y1; y2] e) x1). { now apply Free_Eprim2. }
+            have H' := Hvar _ Hocc H6.
+            destruct H' as [val' [wal' [Hrho [Hloc Hval]]]].
+            exists val', wal'.
+            split. rewrite M.gso; auto.
+            split. 2: now subst fr.
+            destruct Hloc as [i [Hl1 Hl2]].
+            unfold stored_in_locals. exists i. split; auto.
+            subst fr.
+            unfold lookup_N.
+            rewrite set_nth_nth_error_other; auto.
+            intro. assert (x' = i) by lia. subst x'. inv Hrepr_x.
+            specialize Hl1 with err_str.
+            unfold translate_var in Hl1, H8.
+            destruct (lenv ! x1) eqn:Hlx1; rewrite Hlx1 in Hl1=>//. injection Hl1 as ->.
+            destruct (lenv ! x) eqn:Hlx2; rewrite Hlx2 in H8=>//. injection H8 as ->.
+            have H'' := HlenvInjective _ _ _ _ n Hlx2 Hlx1. contradiction.
+            apply nth_error_Some. congruence.
+          }
+        }
+      }
+      exists fr, (Val_unboxed (2 * ord + 1)%N).
+      split. assumption.
+      split. now subst fr.
+      split. assumption.
+      split. assumption.
+      split. assumption.
+      apply rt_step. eapply r_local_set. now subst fr.
+      apply /ssrnat.leP.
+      apply HlocsInBounds in Hrepr_x. lia.
+      now subst fr. }
+
+    unfold load_i64 in Hload1.
+    destruct (load m addr1 0%N 8) eqn:Hload1'. 2: discriminate.
+    assert (addr1 = (Wasm_int.N_of_uint i32m (wasm_value_to_i32 (Val_ptr addr1)))). {
+      cbn. rewrite Wasm_int.Int32.Z_mod_modulus_id. now rewrite N2Z.id.
+      inv Hval_y1; try discriminate. now inv H13. }
+    unfold load_i64 in Hload2.
+    destruct (load m addr2 0%N 8) eqn:Hload2'. 2: discriminate.
+    assert (addr2 = (Wasm_int.N_of_uint i32m (wasm_value_to_i32 (Val_ptr addr2)))). {
+      cbn. rewrite Wasm_int.Int32.Z_mod_modulus_id. now rewrite N2Z.id.
+      inv Hval_y2; try discriminate. now inv H14. }
+
+    have Hreserve1 := Hprim_eq1.
+    destruct Hprim_eq1 as [n1 [i1' [Hn1 [Hw1 [Hi1 Heq_p1']]]]]. subst p1.
+    assert (i1 = i1') by now apply inj_pair2 in Hi1. subst i1'.
+    have Hreserve2 := Hprim_eq2.
+    destruct Hprim_eq2 as [n2 [i2' [Hn2 [Hw2 [Hi2 Heq_p2']]]]]. subst p2.
+    assert (i2 = i2') by now apply inj_pair2 in Hi2. subst i2'.
+
+    assert (Hhalf_modulus: (Wasm_int.Int64.half_modulus = 9223372036854775808)%Z) by
+      now unfold Wasm_int.Int64.half_modulus, Wasm_int.Int64.modulus, two_power_nat.
+
+    assert (HwB: (Wasm_int.Int64.half_modulus = Uint63.wB)%Z) by now unfold Uint63.wB.
+
+    assert (Hunsigned1: Wasm_int.Int64.unsigned w1 = n1). {
+      subst w1. rewrite Wasm_int.Int64.unsigned_repr. reflexivity.
+      unfold Wasm_int.Int64.max_unsigned, Wasm_int.Int64.half_modulus, Wasm_int.Int64.modulus, two_power_nat. now cbn. }
+
+    assert (Hunsigned2: Wasm_int.Int64.unsigned w2 = n2). {
+      subst w2. rewrite Wasm_int.Int64.unsigned_repr. reflexivity.
+      unfold Wasm_int.Int64.max_unsigned, Wasm_int.Int64.half_modulus, Wasm_int.Int64.modulus, two_power_nat. now cbn. }
+
+    assert (Hid1: n1 = Uint63.to_Z i1). {
+      assert (Heqtru: (n1 =? Uint63.to_Z i1)%Z = true) by assumption.
+      by rewrite Z.eqb_eq in Heqtru. }
+    assert (Hid2: n2 = Uint63.to_Z i2). {
+      assert (Heqtru: (n2 =? Uint63.to_Z i2)%Z = true) by assumption.
+      by rewrite Z.eqb_eq in Heqtru. }
+
+    inversion HprimRepr.
+    all: subst x0 y0 y3 p'.
+    all: replace y1'0 with y1' in * by now apply (repr_var_inv lenv y1).
+    all: replace y2'0 with y2' in * by now apply (repr_var_inv lenv y2).
+    {
+      inversion Hprimrel. subst vs f' v1 v2.
+      remember (Wasm_int.Int64.modu (Wasm_int.Int64.iadd w1 w2)
+               (Wasm_int.Int64.repr Wasm_int.Int64.half_modulus)) as w.
+      assert (wasm_i64_prim_related w (AstCommon.primInt; (i1 + i2)%uint63)). {
+        exists ((n1 + n2) mod Wasm_int.Int64.half_modulus)%Z, (i1 + i2)%uint63.
+        try repeat split; try now apply Z.mod_pos_bound.
+        - simpl_modu Heqw. now rewrite -Hunsigned1 -Hunsigned2.
+        - rewrite Uint63.add_spec. now apply Z.eqb_eq. }
+      assert (v = Vprim (AstCommon.primInt; (i1 + i2)%uint63)) by congruence.
+      destruct (H0 _ _ H12 H5) as [s' [s_final [fr [m' [wal [Hs' [Hstore [Hfr [Hsmem [Hstep [Hinv1 [Hupd_glob Hr]]]]]]]]]]]].
+      exists s_final, fr.
+      split. {
+        dostep_nary 0. apply r_global_get. eassumption.
+        eapply rt_trans with (y := (?[hs], ?[sr], ?[f'], ?[s] ++ ?[t])).
+        apply app_trans_const; auto.
+        dostep. apply r_eliml. auto.
+        elimr_nary_instr 2. constructor. apply rs_binop_success. reflexivity.
+        dostep. apply r_eliml. auto.
+        elimr_nary_instr 2. constructor. apply rs_binop_success. cbn.  reflexivity.
+        dostep.
+        elimr_nary_instr 2. eapply r_store_success. cbn in Heqw. now rewrite -Heqw. eassumption. }
+      assumption. }
+    { inversion Hprimrel. subst vs f' v1 v2.
+      remember (Wasm_int.Int64.modu (Wasm_int.Int64.isub w1 w2)
+               (Wasm_int.Int64.repr Wasm_int.Int64.half_modulus)) as w.
+      assert (wasm_i64_prim_related w (AstCommon.primInt; (i1 - i2)%uint63)). {
+        exists ((n1 - n2) mod Wasm_int.Int64.half_modulus)%Z, (i1 - i2)%uint63.
+        try repeat split; try now apply Z.mod_pos_bound.
+        - simpl_modu Heqw. now rewrite -Hunsigned1 -Hunsigned2.
+        - rewrite Uint63.sub_spec. now apply Z.eqb_eq. }
+      assert (v = Vprim (AstCommon.primInt; (i1 - i2)%uint63)) by congruence.
+      destruct (H0 _ _ H12 H5) as [s' [s_final [fr [m' [wal [Hs' [Hstore [Hfr [Hsmem [Hstep [Hinv1 [Hupd_glob Hr]]]]]]]]]]]].
+      exists s_final, fr.
+      split. {
+        dostep_nary 0. apply r_global_get. eassumption.
+        eapply rt_trans with (y := (?[hs], ?[sr], ?[f'], ?[s] ++ ?[t])).
+        apply app_trans_const; auto.
+        dostep. apply r_eliml. auto.
+        elimr_nary_instr 2. constructor. apply rs_binop_success. reflexivity.
+        dostep. apply r_eliml. auto.
+        elimr_nary_instr 2. constructor. apply rs_binop_success. cbn.  reflexivity.
+        dostep.
+        elimr_nary_instr 2. eapply r_store_success. cbn in Heqw. now rewrite -Heqw. eassumption. }
+      assumption. }
+    { inversion Hprimrel. subst vs f' v1 v2.
+      remember (Wasm_int.Int64.modu (Wasm_int.Int64.imul w1 w2)
+               (Wasm_int.Int64.repr Wasm_int.Int64.half_modulus)) as w.
+      assert (wasm_i64_prim_related w (AstCommon.primInt; (i1 * i2)%uint63)). {
+        exists ((n1 * n2) mod Wasm_int.Int64.half_modulus)%Z, (i1 * i2)%uint63.
+        try repeat split; try now apply Z.mod_pos_bound.
+        - simpl_modu Heqw. now rewrite -Hunsigned1 -Hunsigned2.
+        - rewrite Uint63.mul_spec. now apply Z.eqb_eq. }
+      assert (v = Vprim (AstCommon.primInt; (i1 * i2)%uint63)) by congruence.
+      destruct (H0 _ _ H12 H5) as [s' [s_final [fr [m' [wal [Hs' [Hstore [Hfr [Hsmem [Hstep [Hinv1 [Hupd_glob Hr]]]]]]]]]]]].
+      exists s_final, fr.
+      split. {
+        dostep_nary 0. apply r_global_get. eassumption.
+        eapply rt_trans with (y := (?[hs], ?[sr], ?[f'], ?[s] ++ ?[t])).
+        apply app_trans_const; auto.
+        dostep. apply r_eliml. auto.
+        elimr_nary_instr 2. constructor. apply rs_binop_success. reflexivity.
+        dostep. apply r_eliml. auto.
+        elimr_nary_instr 2. constructor. apply rs_binop_success. cbn.  reflexivity.
+        dostep.
+        elimr_nary_instr 2. eapply r_store_success. cbn in Heqw. now rewrite -Heqw. eassumption. }
+      assumption. }
+    { inversion Hprimrel. subst vs f' v1 v2.
+      destruct (Wasm_int.Int64.eq_dec w2 Wasm_int.Int64.zero) eqn:Hzero. {
+        assert (wasm_i64_prim_related Wasm_int.Int64.zero (AstCommon.primInt; (i1 / i2)%uint63)). {
+          exists 0%Z, 0%uint63.
+          assert (n2 = 0)%Z. {
+            unfold Wasm_int.Int64.zero in e0. rewrite e0 in Hw2.
+            apply Wasm_int.Int64.repr_inv in Hw2. symmetry. assumption.
+            unfold Wasm_int.Int64.modulus, Wasm_int.Int64.half_modulus, two_power_nat. cbn. lia.
+            unfold Wasm_int.Int64.modulus, Wasm_int.Int64.half_modulus, two_power_nat. cbn.
+            unfold Wasm_int.Int64.modulus, Wasm_int.Int64.half_modulus, two_power_nat in Hn2. cbn in Hn2. lia. }
+          assert (Uint63.to_Z 0 = 0%Z)%uint63 by now simpl.
+          assert (i2 = 0)%uint63. {
+            rewrite H5 in Hid2.
+            rewrite -H12 in Hid2.
+            now apply Uint63.to_Z_inj in Hid2. } subst i2.
+          assert (i1 / 0 = of_Z (to_Z (i1 / 0)))%uint63 by now rewrite Uint63.of_to_Z.
+          assert (to_Z (i1 / 0) = 0%Z). {
+            rewrite Uint63.div_spec.
+            rewrite H12. unfold Z.div. unfold Z.div_eucl.
+            destruct (Uint63.to_Z i1); reflexivity. }
+          assert (i1 / 0 = 0)%uint63. {
+            rewrite H13.
+            rewrite Uint63.div_spec.
+            rewrite Uint63.div_spec in H14.
+            rewrite H14. reflexivity. }
+          try repeat split.
+          - lia.
+          - now rewrite H15. }
+        assert (v = Vprim (AstCommon.primInt; (i1 / i2)%uint63)) by congruence.
+        destruct (H0 _ _ H12 H5) as [s' [s_final [fr [m' [wal [Hs' [Hstore [Hfr [Hsmem [Hstep [Hinv1 [Hupd_glob Hr]]]]]]]]]]]].
+        exists s_final, fr.
+        split. {
+        dostep_nary 0. apply r_local_get. eassumption.
+        dostep_nary 1. eapply r_load_success; try eassumption. subst wal2. rewrite -H4. apply Hload2'.
+        replace (wasm_deserialise b0 T_i64) with (VAL_int64 w2) by congruence.
+        dostep_nary 1. constructor. apply rs_testop_i64.
+        dostep_nary 1. constructor. apply rs_if_true. unfold wasm_bool. cbn. unfold Wasm_int.Int64.zero. rewrite e0. cbn. discriminate.
+        dostep_nary 0. eapply r_block with (t1s:=[::]) (t2s:=[::])(vs:=[::]); auto. cbn.
+        separate_instr.
+        assert (forall es,
+                   reduce_trans (state, s, f,
+                       ([:: AI_label 0 [::]
+                          ([:: AI_basic (BI_global_get global_mem_ptr)] ++
+                             [:: $VN nat_to_value64 0] ++ [:: AI_basic (BI_store T_i64 None 2%N 0%N)])] ++ es))
+                     (state, s', f, es)). {
+          intros.
+          eapply rt_trans.
+          apply app_trans.
+          apply reduce_trans_label.
+          dostep_nary 0. apply r_global_get. eassumption.
+          dostep'. eapply r_store_success.
+          unfold nat_to_value64. unfold nat_to_i64. unfold Z.of_nat. unfold Wasm_int.Int64.zero in Hstore. eassumption. apply rt_refl. apply rt_refl. }
+        eapply rt_trans.
+        apply H13.
+        apply Hstep. }
+      assumption. } {
+        assert (wasm_i64_prim_related (Wasm_int.Int64.divu w1 w2) (AstCommon.primInt; (i1 / i2)%uint63)). {
+          exists (n1 / n2)%Z, (Uint63.div i1 i2).
+          assert (n2 <> 0)%Z. {
+            intro Hcontra.
+            subst w2.
+            unfold Wasm_int.Int64.zero in n3.
+            now unfold "<>" in n3. }
+          try repeat split.
+          - apply Z.div_pos; lia.
+          - apply Z.div_lt_upper_bound; lia.
+          - unfold Wasm_int.Int64.divu. now rewrite Hunsigned1 Hunsigned2.
+          - rewrite Uint63.div_spec.
+            now apply Z.eqb_eq. }
+        assert (v = Vprim (AstCommon.primInt; (i1 / i2)%uint63)) by congruence.
+        destruct (H0 _ _ H12 H5) as [s' [s_final [fr [m' [wal [Hs' [Hstore [Hfr [Hsmem [Hstep [Hinv1 [Hupd_glob Hr]]]]]]]]]]]].
+        exists s_final, fr.
+        split. {
+          dostep_nary 0. apply r_local_get. eassumption.
+          dostep_nary 1. eapply r_load_success; try eassumption. subst wal2. rewrite -H4. apply Hload2'.
+          replace (wasm_deserialise b0 T_i64) with (VAL_int64 w2) by congruence.
+          dostep_nary 1. constructor. apply rs_testop_i64.
+          dostep_nary 1. constructor. apply rs_if_false. unfold wasm_bool. cbn.
+          assert (Wasm_int.Int64.eq Wasm_int.Int64.zero w2 = false) by now apply Wasm_int.Int64.eq_false. now rewrite H13.
+          dostep_nary 0. eapply r_block with (t1s:=[::]) (t2s:=[::])(vs:=[::]); auto. cbn.
+          separate_instr.
+          eapply rt_trans.
+          apply app_trans.
+          apply reduce_trans_label.
+          dostep_nary 0. apply r_global_get. eassumption.
+          eapply rt_trans with (y := (?[hs], ?[sr], ?[f'], ?[s] ++ ?[t])).
+          apply app_trans_const; auto.
+          dostep. apply r_eliml. auto.
+          elimr_nary_instr 2. constructor. apply rs_binop_success.
+          cbn. unfold Wasm_int.Int64.idiv_u.
+          assert (Wasm_int.Int64.eq w2 Wasm_int.Int64.zero = false) by now apply Wasm_int.Int64.eq_false.
+          now rewrite H13.
+          dostep'. elimr_nary_instr 2. eapply r_store_success; eassumption.
+          now apply rt_refl.
+          now apply Hstep. }
+        assumption. } }
+    { inversion Hprimrel. subst vs f' v1 v2.
+      remember (Wasm_int.Int64.modu (Wasm_int.Int64.iand w1 w2)
+               (Wasm_int.Int64.repr Wasm_int.Int64.half_modulus)) as w.
+      assert (wasm_i64_prim_related w (AstCommon.primInt; (i1 land i2)%uint63)). {
+            assert ((Z.land n1 n2) = Uint63.to_Z (Uint63.land i1 i2))%Z. {
+              rewrite Uint63.land_spec'. now rewrite Hid1 Hid2. }
+            assert (0 <= Z.land n1 n2 < Wasm_int.Int64.half_modulus)%Z. {
+              rewrite HwB. rewrite H5. now apply Uint63.to_Z_bounded. }
+            assert (0 <= Z.land n1 n2 < Wasm_int.Int64.modulus)%Z. {
+              unfold Wasm_int.Int64.modulus, Wasm_int.Int64.half_modulus, two_power_nat. cbn.
+              unfold Wasm_int.Int64.modulus, Wasm_int.Int64.half_modulus, two_power_nat in H12. cbn in H12. lia. }
+        exists (Z.land n1 n2)%Z, (Uint63.land i1 i2).
+        try repeat split.
+        - now apply Z.land_nonneg.
+        - rewrite H5. now apply Uint63.to_Z_bounded.
+        - subst w. unfold Wasm_int.Int64.iand, Wasm_int.Int64.and.
+          rewrite Hunsigned1 Hunsigned2.
+          unfold Wasm_int.Int64.modu.
+          assert (Wasm_int.Int64.unsigned (Wasm_int.Int64.repr (Z.land n1 n2)) = Z.land n1 n2). {
+            cbn. rewrite Wasm_int.Int64.Z_mod_modulus_id. reflexivity. lia. }
+          rewrite H14.
+          cbn.
+          rewrite Zmod_small. reflexivity. assumption.
+        - now apply Z.eqb_eq. }
+      assert (v = Vprim (AstCommon.primInt; (i1 land i2)%uint63)) by congruence.
+      destruct (H0 _ _ H12 H5) as [s' [s_final [fr [m' [wal [Hs' [Hstore [Hfr [Hsmem [Hstep [Hinv1 [Hupd_glob Hr]]]]]]]]]]]].
+      exists s_final, fr.
+      split. {
+        dostep_nary 0. apply r_global_get. eassumption.
+        eapply rt_trans with (y := (?[hs], ?[sr], ?[f'], ?[s] ++ ?[t])).
+        apply app_trans_const; auto.
+        dostep. apply r_eliml. auto.
+        elimr_nary_instr 2. constructor. apply rs_binop_success. reflexivity.
+        dostep. apply r_eliml. auto.
+        elimr_nary_instr 2. constructor. apply rs_binop_success. cbn.  reflexivity.
+        dostep.
+        elimr_nary_instr 2. eapply r_store_success. cbn in Heqw. now rewrite -Heqw. eassumption. }
+      assumption. }
+    { inversion Hprimrel. subst vs f' v1 v2.
+      remember (Wasm_int.Int64.modu (Wasm_int.Int64.ior w1 w2)
+               (Wasm_int.Int64.repr Wasm_int.Int64.half_modulus)) as w.
+      assert (wasm_i64_prim_related w (AstCommon.primInt; (i1 lor i2)%uint63)). {
+            assert ((Z.lor n1 n2) = Uint63.to_Z (Uint63.lor i1 i2))%Z. {
+              rewrite Uint63.lor_spec'. now rewrite Hid1 Hid2. }
+            assert (0 <= Z.lor n1 n2 < Wasm_int.Int64.half_modulus)%Z. {
+              rewrite HwB. rewrite H5. now apply Uint63.to_Z_bounded. }
+            assert (0 <= Z.lor n1 n2 < Wasm_int.Int64.modulus)%Z. {
+              unfold Wasm_int.Int64.modulus, Wasm_int.Int64.half_modulus, two_power_nat. cbn.
+              unfold Wasm_int.Int64.modulus, Wasm_int.Int64.half_modulus, two_power_nat in H12. cbn in H12. lia. }
+        exists (Z.lor n1 n2)%Z, (Uint63.lor i1 i2).
+        try repeat split.
+            - now apply Z.lor_nonneg; lia.
+            - lia.
+        - subst w. unfold Wasm_int.Int64.ior, Wasm_int.Int64.or.
+          rewrite Hunsigned1 Hunsigned2.
+          unfold Wasm_int.Int64.modu.
+          assert (Wasm_int.Int64.unsigned (Wasm_int.Int64.repr (Z.lor n1 n2)) = Z.lor n1 n2). {
+            cbn. rewrite Wasm_int.Int64.Z_mod_modulus_id. reflexivity. lia. }
+          rewrite H14.
+          cbn.
+          rewrite Zmod_small. reflexivity. assumption.
+        - now apply Z.eqb_eq. }
+      assert (v = Vprim (AstCommon.primInt; (i1 lor i2)%uint63)) by congruence.
+      destruct (H0 _ _ H12 H5) as [s' [s_final [fr [m' [wal [Hs' [Hstore [Hfr [Hsmem [Hstep [Hinv1 [Hupd_glob Hr]]]]]]]]]]]].
+      exists s_final, fr.
+      split. {
+        dostep_nary 0. apply r_global_get. eassumption.
+        eapply rt_trans with (y := (?[hs], ?[sr], ?[f'], ?[s] ++ ?[t])).
+        apply app_trans_const; auto.
+        dostep. apply r_eliml. auto.
+        elimr_nary_instr 2. constructor. apply rs_binop_success. reflexivity.
+        dostep. apply r_eliml. auto.
+        elimr_nary_instr 2. constructor. apply rs_binop_success. cbn.  reflexivity.
+        dostep.
+        elimr_nary_instr 2. eapply r_store_success. cbn in Heqw. now rewrite -Heqw. eassumption. }
+      assumption. }
+    { inversion Hprimrel. subst vs f' v1 v2.
+      remember (Wasm_int.Int64.modu (Wasm_int.Int64.ishl w1 w2)
+               (Wasm_int.Int64.repr Wasm_int.Int64.half_modulus)) as w.
+      assert (wasm_i64_prim_related w (AstCommon.primInt; (i1 << i2)%uint63)). {
+        exists ((Z.shiftl n1 n2) mod Wasm_int.Int64.half_modulus)%Z, (Uint63.lsl i1 i2).
+        try repeat split; try apply Z.mod_pos_bound; try lia.
+        - simpl_modu Heqw. now rewrite -Hunsigned1 -Hunsigned2.
+        - rewrite Uint63.lsl_spec.
+          rewrite -Hid1 -Hid2.
+          rewrite Z.shiftl_mul_pow2.
+          now apply Z.eqb_eq.
+          lia. }
+      assert (v = Vprim (AstCommon.primInt; (i1 << i2)%uint63)) by congruence.
+      destruct (H0 _ _ H12 H5) as [s' [s_final [fr [m' [wal [Hs' [Hstore [Hfr [Hsmem [Hstep [Hinv1 [Hupd_glob Hr]]]]]]]]]]]].
+      exists s_final, fr.
+      split. {
+        dostep_nary 0. apply r_global_get. eassumption.
+        eapply rt_trans with (y := (?[hs], ?[sr], ?[f'], ?[s] ++ ?[t])).
+        apply app_trans_const; auto.
+        dostep. apply r_eliml. auto.
+        elimr_nary_instr 2. constructor. apply rs_binop_success. reflexivity.
+        dostep. apply r_eliml. auto.
+        elimr_nary_instr 2. constructor. apply rs_binop_success. cbn.  reflexivity.
+        dostep.
+        elimr_nary_instr 2. eapply r_store_success. cbn in Heqw. now rewrite -Heqw. eassumption. }
+      assumption. }
+    { inversion Hprimrel. subst vs f' v1 v2.
+      remember (Wasm_int.Int64.modu (Wasm_int.Int64.ishr_u w1 w2)
+               (Wasm_int.Int64.repr Wasm_int.Int64.half_modulus)) as w.
+      assert (wasm_i64_prim_related w (AstCommon.primInt; (i1 >> i2)%uint63)). {
+        exists ((Z.shiftr n1 n2) mod Wasm_int.Int64.half_modulus)%Z, (Uint63.lsr i1 i2).
+        assert ((Z.shiftr n1 n2) = Uint63.to_Z (Uint63.lsr i1 i2))%Z. {
+          rewrite Uint63.lsr_spec.
+          rewrite -Hid1 -Hid2.
+          apply Z.shiftr_div_pow2. lia.
+        }
+        try repeat split; try apply Z.mod_pos_bound; try lia.
+        - simpl_modu Heqw. now rewrite -Hunsigned1 -Hunsigned2.
+        - rewrite Uint63.lsr_spec.
+          rewrite -Hid1 -Hid2.
+          rewrite Zmod_small. rewrite Z.shiftr_div_pow2.
+          now apply Z.eqb_eq. lia.
+          rewrite H5. now apply Uint63.to_Z_bounded. }
+      assert (v = Vprim (AstCommon.primInt; (i1 >> i2)%uint63)) by congruence.
+      destruct (H0 _ _ H12 H5) as [s' [s_final [fr [m' [wal [Hs' [Hstore [Hfr [Hsmem [Hstep [Hinv1 [Hupd_glob Hr]]]]]]]]]]]].
+      exists s_final, fr.
+      split. {
+        dostep_nary 0. apply r_global_get. eassumption.
+        eapply rt_trans with (y := (?[hs], ?[sr], ?[f'], ?[s] ++ ?[t])).
+        apply app_trans_const; auto.
+        dostep. apply r_eliml. auto.
+        elimr_nary_instr 2. constructor. apply rs_binop_success. reflexivity.
+        dostep. apply r_eliml. auto.
+        elimr_nary_instr 2. constructor. apply rs_binop_success. cbn.  reflexivity.
+        dostep.
+        elimr_nary_instr 2. eapply r_store_success. cbn in Heqw. now rewrite -Heqw. eassumption. }
+      assumption. }
+    { inversion Hprimrel. subst vs f' v1 v2.
+      destruct (Wasm_int.Int64.eq_dec w1 w2) eqn:Heq. {
+        assert ((i1 =? i2)%uint63 = true). {
+          rewrite -e0 in Hreserve2.
+          assert ((AstCommon.primInt ; i1) = (AstCommon.primInt ; i2)) by now apply prim_rel_inv with (w:=w1).
+          apply inj_pair2 in H7. subst i2. now apply Uint63.eqb_spec. }
+        rewrite H7 in HprimResSome.
+        assert (v = Vconstr t_true []) by congruence.
+        assert (get_ctor_ord cenv t_true = Ret 0%N). { unfold get_ctor_ord. now rewrite H12. }
+        assert (get_ctor_arity cenv t_true = Ret 0). { unfold get_ctor_arity. now rewrite H12. }
+        destruct (H2 _ _ H14 H16 H15) as [fr [wal [Hinv' [Hfr [HreprVal [HrelE' [HvalsPreserved Hstep]]]]]]].
+        exists s, fr.
+        split. {
+          separate_instr.
+          eapply rt_trans with (y := (?[hs], ?[sr], ?[f'], ?[s] ++ ?[t])).
+          apply HloadStep.
+          dostep. elimr_nary_instr 2. constructor. apply rs_relop.
+          dostep_nary 1. constructor. apply rs_if_true.
+          rewrite e0. unfold wasm_bool.
+          assert (Wasm_int.Int64.eq w2 w2 = true) by now apply Wasm_int.Int64.eq_true. now rewrite H17.
+          dostep_nary 0. eapply r_block with (t1s:=[::]) (t2s:=[:: T_num T_i32])(vs:=[::]); eauto.
+          dostep_nary 0. constructor. apply rs_label_const; auto.
+          assert ([:: $VN nat_to_value 1] = [:: $V VAL_num (VAL_int32 (wasm_value_to_i32 wal))]). {
+            assert (wal = Val_unboxed 1%N). { inv HreprVal; try discriminate. inv H21. now replace ord with 0%N by congruence. inv H28. rewrite H16 in H20. now inv H21. }
+            now rewrite H17. }
+          rewrite H17.
+          now apply Hstep. }
+        split. assumption.
+        split. now subst fr.
+        split. reflexivity.
+        split. assumption.
+        split. assumption.
+        exists wal.
+        split. now subst fr.
+        split. unfold stored_in_locals. exists x'. split. intros. inv Hrepr_x. unfold translate_var. unfold translate_var in H17. destruct (lenv ! x) eqn:Hx. rewrite Hx in H17. rewrite Hx. congruence. now rewrite Hx in H17.
+        subst fr. cbn. unfold lookup_N. apply nth_error_set_eq.
+        now subst fr. } {
+        assert ((i1 =? i2)%uint63 = false). {
+          (* inversion Hprim_eq1. *)
+          (* destruct H5 as [i1' [Hn1 [Hn1' [Hi1' Heq1']]]]. *)
+          (* inversion Hprim_eq2. *)
+          (* destruct H5 as [i2' [Hn2 [Hn2' [Hi2' Heq']]]]. *)
+          (* apply inj_pair2 in Hi1'. apply inj_pair2 in Hi2'. subst i1' i2'. *)
+          rewrite Uint63.eqb_false_spec.
+          assert (n1 <> n2). {
+            intro Hcontra. unfold not in n3.
+            subst w1 w2. apply n3. now subst n1. }
+          (* assert (n2 =? to_Z i2 = true)%Z by assumption. *)
+          (* assert (n1 =? to_Z i1 = true)%Z by assumption. *)
+          (* rewrite Z.eqb_eq in H6. *)
+          (* rewrite Z.eqb_eq in H7. *)
+          rewrite Hid1 in H7. rewrite Hid2 in H7.
+          unfold not in H7.
+          intro Hcontra.
+          assert (to_Z i1 = to_Z i2) by congruence. now apply H7 in H14. }
+        rewrite H7 in HprimResSome.
+        assert (v = Vconstr t_false []) by congruence.
+        assert (get_ctor_ord cenv t_false = Ret 1%N). { unfold get_ctor_ord. now rewrite H13. }
+        assert (get_ctor_arity cenv t_false = Ret 0). { unfold get_ctor_arity. now rewrite H13. }
+        destruct (H2 _ _ H14 H16 H15) as [fr [wal [Hinv' [Hfr [HreprVal [HrelE' [HvalsPreserved Hstep]]]]]]].
+        exists s, fr.
+        split. {
+          separate_instr.
+          eapply rt_trans with (y := (?[hs], ?[sr], ?[f'], ?[s] ++ ?[t])).
+          apply HloadStep.
+          dostep. elimr_nary_instr 2. constructor. apply rs_relop.
+          dostep_nary 1. constructor. apply rs_if_false.
+          unfold wasm_bool.
+          assert (Wasm_int.Int64.eq w1 w2 = false) by now apply Wasm_int.Int64.eq_false.
+          now rewrite H17.
+          dostep_nary 0. eapply r_block with (t1s:=[::]) (t2s:=[:: T_num T_i32])(vs:=[::]); eauto.
+          dostep_nary 0. constructor. apply rs_label_const; auto.
+          assert ([:: $VN nat_to_value 3] = [:: $V VAL_num (VAL_int32 (wasm_value_to_i32 wal))]). {
+            assert (wal = Val_unboxed 3%N). { inv HreprVal; try discriminate. inv H21. now replace ord with 1%N by congruence. inv H28. rewrite H16 in H20. now inv H20. }
+            now rewrite H17. }
+          rewrite H17.
+          now apply Hstep. }
+        split. assumption.
+        split. now subst fr.
+        split. reflexivity.
+        split. assumption.
+        split. assumption.
+        exists wal.
+        split. now subst fr.
+        split. unfold stored_in_locals. exists x'. split. intros. inv Hrepr_x. unfold translate_var. unfold translate_var in H17. destruct (lenv ! x) eqn:Hx. rewrite Hx in H17. rewrite Hx. congruence. now rewrite Hx in H17.
+        subst fr. cbn. unfold lookup_N. apply nth_error_set_eq.
+        now subst fr. } }
 Qed.
 
 Close Scope bs_scope.
